Cleaned-up embarrassing comments / simplified proof

easycrypt/KEM.ec
@@ -1,11 +1,17 @@
 (*
- * Proof of Theorem 2 in the Technical Report
+ * Proof of Theorem 1
  *
  * Theorem: if the pre-master secret KEM used in the TLS handshake is
  * both One-Way and Non-Randomizable under Plaintext-Checking Attacks,
  * then the master secret KEM, seen as an agile labeled KEM, is
  * Indistinguishable under Replayable Chosen-Ciphertext Attacks in the
  * ROM for the underlying agile KEF.
+ *
+ * The definition of the master secret KEM includes the countermeasure
+ * against padding-oracle attacks (aka Bleichenbecher attacks) used for
+ * RSA encryption with PKCS#1 padding: when decryption fails, a value for
+ * the master secret is computed anyway using a random pre-master secret.
+ *
  *)
 
 require import Bool.
@@ -13,9 +19,15 @@ require import Int.
 require import Real.
 require import Pair.
 require import FMap.
+require import ISet.
+require import RandomOracle.
 
+import Finite.
 import FSet.
 import OptionGet.
+
+(* Bare minimum *)
+prover "Alt-Ergo" "Z3".
 
 lemma eq_except_in_dom (m1 m2:('a, 'b) map) (x y:'a) :
   eq_except m1 m2 x => x <> y => (in_dom y m1 <=> in_dom y m2) 
@@ -25,8 +37,6 @@ lemma eq_except_set (m1 m2:('a, 'b) map) (x y:'a) (z:'b) :
   eq_except m1 m2 x => eq_except m1.[y <- z] m2.[y <- z] x 
 by [].
 
-
-(* TODO: Map this to a RO in the standard library *)
 theory Agile_KEF.
 
   type parameter.
@@ -57,15 +67,15 @@ theory Agile_Labeled_KEM.
     fun init() : unit {*}
     fun keygen() : pkey * skey
     fun enc(p:parameter, pk:pkey, t:label) : key * ciphertext
-    fun dec(p:parameter, sk:skey, t:label, c:ciphertext) : key
+    fun dec(p:parameter, sk:skey, t:label, c:ciphertext) : key option
   }.
 
   theory RCCA.
   
     const P : parameter set.
    
-    const pp : parameter.
-   
+    const pp : parameter. 
+     
     op key : key distr.
      
     module type Oracle = {
@@ -81,6 +91,8 @@ theory Agile_Labeled_KEM.
       var sk : skey
       var keys : key set
       var labels : label set
+      var guess : bool
+      var t : label
     }.
     
     module Wrap(KEM:KEM) : Oracle = {  
@@ -89,8 +101,10 @@ theory Agile_Labeled_KEM.
         var maybe_k : key option = None;
         if (!mem t W.labels /\ mem p P) { 
           W.labels = add t W.labels;
-          k = KEM.dec(p, W.sk, t, c);
-          maybe_k = if (!mem k W.keys) then Some k else None;
+          maybe_k = KEM.dec(p, W.sk, t, c);
+          maybe_k = 
+           if (W.guess => !mem (proj maybe_k) W.keys \/ t <> W.t) 
+           then maybe_k else None;
         }
         return maybe_k;
       }
@@ -104,25 +118,26 @@ theory Agile_Labeled_KEM.
         var b, b', valid : bool;
         var k0, k1 : key;
         var c : ciphertext;
-        var t : label;
         var pk : pkey;
         KEM.init();
         (pk, W.sk) = KEM.keygen();
         W.keys = FSet.empty;
         W.labels = FSet.empty;
-        t = A.choose(pk);
-        valid = !mem t W.labels; 
-        (k0, c) = KEM.enc(pp, pk, t);
+        W.t = pick FSet.empty;
+        W.guess = false;
+        W.t = A.choose(pk);
+        valid = !mem W.t W.labels; 
+        (k0, c) = KEM.enc(pp, pk, W.t);
         k1 = $key;
         b = ${0,1};
         W.keys = add k0 (add k1 W.keys);
+        W.guess = true;
         b' = A.guess(c, if b then k1 else k0);
         return (b = b' /\ valid);
       }
     }.
   
   end RCCA.
-  
   
   theory PCA.
   
@@ -143,12 +158,12 @@ theory Agile_Labeled_KEM.
     
     module Wrap(KEM:KEM) : Oracle = {
       fun check(p:parameter, k:key, t:label, c:ciphertext) : bool = {
-        var k' : key;
-        k' = KEM.dec(p, V.sk, t, c);
-        return (k' = k);
+        var maybe_k : key option;
+        maybe_k = KEM.dec(p, V.sk, t, c);
+        return (maybe_k = Some k);
       }
     }.
-      
+
     module OW_PCA(KEM:KEM, A:OW_Adversary) = {
       module O = Wrap(KEM)
       module A = A(O)
@@ -169,7 +184,7 @@ theory Agile_Labeled_KEM.
 
     module type NR_Adversary(O:Oracle) = {
       fun choose(pk:pkey) : label
-      fun guess(c:ciphertext) : label * ciphertext
+      fun guess(c:ciphertext) : ciphertext
     }.
    
     module NR_PCA(KEM:KEM, A:NR_Adversary) = {
@@ -178,16 +193,18 @@ theory Agile_Labeled_KEM.
     
       fun main() : bool = {
         var pk : pkey;
-        var t, t' : label;
-        var k, k' : key;
+        var t : label;
+        var p : parameter;
+        var k : key;
+        var maybe_k : key option;
         var c, c' : ciphertext;
         KEM.init();
         (pk, V.sk) = KEM.keygen();
         t = A.choose(pk);
         (k, c) = KEM.enc(pp, pk, t);
-        (t', c') = A.guess(c);
-        k' = KEM.dec(pp, V.sk, t', c');
-        return (c <> c' /\ k' = k);
+        c' = A.guess(c);
+        maybe_k = KEM.dec(pp, V.sk, t, c');
+        return (c <> c' /\ maybe_k = Some k);
       }
     }.
   
@@ -206,28 +223,40 @@ op key : ms distr.
 
 axiom key_lossless : Distr.weight key = 1%r.
 
-(* Shall we treat pv as a label or as a parameter? As a label for now *)
-(* Theory for non-agile pre-master secret KEM with protocol version as label *)
-clone import Agile_Labeled_KEM as Inner_KEM with 
-  type parameter <- unit,
-  type label     <- version,
-  type key       <- pms.
+op dpms : version -> pms distr.
+
+axiom dpms_lossless : forall pv, Distr.weight (dpms pv) = 1%r.
 
 (* Theory for agile and labeled master-secret KEM *)
-clone Agile_Labeled_KEM as Outer_KEM with 
+clone import Agile_Labeled_KEM as Outer_KEM with 
   type parameter  <- version * hash,
   type label      <- label,
   type key        <- ms,
-  type pkey       <- Inner_KEM.pkey,
-  type skey       <- Inner_KEM.skey,
-  type ciphertext <- Inner_KEM.ciphertext,
   op RCCA.key     <- key.
+
+(* Theory for pre-master secret KEM with protocol version as agility param. *)
+clone Agile_Labeled_KEM as Inner_KEM with 
+  type parameter  <- version,
+  type pkey       <- Outer_KEM.pkey,
+  type skey       <- Outer_KEM.skey,
+  type ciphertext <- Outer_KEM.ciphertext,
+  type label      <- unit,
+  type key        <- pms,
+  op PCA.pp       <- fst Outer_KEM.RCCA.pp.
+
+import Inner_KEM.
 
 (* Theory for agile KEF, indexed by a hash algorithm identifier *)
 clone Agile_KEF as KEF with
-  type parameter <- hash,
+  type parameter <- version * hash,
   type secret    <- pms * label,
   type key       <- ms.
+
+(* Used for the transformation from RCCA0 to RCCA1 *)
+clone LazyEager as LE with 
+  type from  <- version * label,
+  type to    <- pms,
+  op dsample <- lambda (p:version * label), dpms (fst p).
 
 (* TLS master secret KEM *)
 module KEM(KEF:KEF.KEF, PMS_KEM:Inner_KEM.KEM) : Outer_KEM.KEM = {
@@ -250,33 +279,36 @@ module KEM(KEF:KEF.KEF, PMS_KEM:Inner_KEM.KEM) : Outer_KEM.KEM = {
     var pv : version;
     var h : hash;
     (pv, h) = p;
-    (pms, c) = PMS_KEM.enc((), pk, pv);
-    ms = KEF.extract(h, (pms, t));
+    (pms, c) = PMS_KEM.enc(pv, pk, ());
+    ms = KEF.extract((pv, h), (pms, t));
     return (ms, c);
   }
 
-  fun dec(p:version * hash, sk:skey, t:label, c:ciphertext) : ms = {
+  fun dec(p:version * hash, sk:skey, t:label, c:ciphertext) : ms option = {
+    var maybe_pms : pms option;
     var pms : pms;
     var ms : ms;
     var pv : version;
     var h : hash;
     (pv, h) = p;
-    pms = PMS_KEM.dec((), sk, pv, c);
-    ms = KEF.extract(h, (pms, t));
-    return ms;
+    maybe_pms = PMS_KEM.dec(pv, sk, (), c);
+    pms = $dpms pv;
+    pms = if maybe_pms = None then pms else proj maybe_pms;
+    ms = KEF.extract((pv, h), (pms, t));
+    return Some ms;
   }
 }.
 
 
 (* Agile KEF in the ROM *)
 module RO_KEF : KEF.KEF = {
-  var m : (hash * (pms * label), ms) map
+  var m : ((version * hash) * (pms * label), ms) map
  
   fun init() : unit = {
     m = Core.empty;
   }
  
-  fun extract(p:hash, s:pms * label) : ms = {
+  fun extract(p:version * hash, s:pms * label) : ms = {
     if (!in_dom (p, s) m) m.[(p, s)] = $key;
     return proj m.[(p, s)];
   }
@@ -298,79 +330,67 @@ module type Adversary(O1:KEF.Oracle, O2:Oracle) = {
 
 section.
 
-  declare module PMS_KEM : Inner_KEM.KEM {RO_KEF, RCCA, PCA.NR_PCA, PCA.OW_PCA}.
+  declare module PMS_KEM : Inner_KEM.KEM {RO_KEF, RCCA, PCA.NR_PCA, PCA.OW_PCA, LE.Lazy.RO, LE.Eager.RO}.
 
   (* Assumptions on the Pre-master secret KEM *)
+  axiom stateless_pms_kem (x y:glob PMS_KEM) : x = y.
 
-  (* 
-   * REMARK: This can be weakened. It is enough to require that 
-   * PMS_KEM.enc and PMS_KEM.dec do not write shared global state
-   * (read-only shared state initialized by PMS_KEM.init and 
-   * PMS_KEM.keygen is fine).
-   *)
-  axiom stateless_pms_kem : forall (x y:glob PMS_KEM), x = y.
+  axiom finite_labels : finite univ<:label>.
 
-  (* TODO: maybe move the first 2 operators to PMS_KEM *)
+  axiom finite_pms : finite univ<:pms>.
+
   op keypair : pkey * skey -> bool.
 
-  op decrypt : skey -> version -> ciphertext -> pms.
-
-  op same_key : pkey -> version -> version -> ciphertext -> bool.
-
-  (* 
-   * REMARK: The axiom previously used only holds for RSA:
-   *
-   * axiom nosmt dec_injective_pv : forall sk pv1 pv2 c,
-   * decrypt sk pv1 c = decrypt sk pv2 c => pv1 = pv2.
-   *
-   * For RSA, same_key pk pv1 pv2 c := pv1 = pv2
-   * For DH, same_key pk pv1 pv2 c := true
-   *)  
-  axiom nosmt same_key_spec : forall pk sk pv1 pv2 c,
-    keypair(pk, sk) =>
-    (same_key pk pv1 pv2 c <=> decrypt sk pv1 c = decrypt sk pv2 c).
+  op decrypt : version -> skey -> ciphertext -> pms option.
 
   axiom keygen_spec_rel :
     equiv [ PMS_KEM.keygen ~ PMS_KEM.keygen : true ==> ={res} /\ keypair res{1} ].
 
-  axiom enc_spec_rel : forall sk pk pv,
+  axiom enc_spec_rel sk pk pv :
     equiv [ PMS_KEM.enc ~ PMS_KEM.enc :
-      pk{1} = pk /\ t{1} = pv /\ ={pk, t} /\ keypair(pk, sk) ==>
-      ={res} /\ let (k, c) = res{1} in decrypt sk pv c = k ].
+      p{1} = pv /\ pk{1} = pk /\ ={pk, t} /\ keypair(pk, sk) ==>
+      ={res} /\ let (k, c) = res{1} in decrypt pv sk c = Some k ].
 
-  axiom dec_spec : forall _sk _pv _c,
+  axiom dec_spec _sk _pv _c :
     bd_hoare [ PMS_KEM.dec :
-      sk = _sk /\ t = _pv /\ c = _c ==> res = decrypt _sk _pv _c ] = 1%r.
+      p = _pv /\ sk = _sk /\ c = _c ==> res = decrypt _pv _sk _c ] = 1%r.
   
   (* TLS master secret KEM in the ROM for KEF *)
   local module MS_KEM = KEM(RO_KEF, PMS_KEM).
 
   (* RCCA adversary *)
-  declare module A : Adversary
-    {RO_KEF, PMS_KEM, RCCA, PCA.NR_PCA, PCA.OW_PCA}.
+  declare module A : Adversary {RO_KEF, PMS_KEM, RCCA, PCA.NR_PCA, PCA.OW_PCA, LE.Lazy.RO, LE.Eager.RO}.
 
-  axiom lossless_choose : 
-    forall (O1 <: KEF.Oracle {A}) (O2 <: Oracle {A}),
-      islossless O2.dec => islossless O1.extract => islossless A(O1, O2).choose.
+  axiom lossless_choose (O1 <: KEF.Oracle {A}) (O2 <: Oracle {A}) :
+   islossless O2.dec => islossless O1.extract => islossless A(O1, O2).choose.
 
-  axiom lossless_guess : 
-    forall (O1 <: KEF.Oracle {A}) (O2 <: Oracle {A}),
-      islossless O2.dec => islossless O1.extract => islossless A(O1, O2).guess.
-   
+  axiom lossless_guess (O1 <: KEF.Oracle {A}) (O2 <: Oracle {A}) :
+    islossless O2.dec => islossless O1.extract => islossless A(O1, O2).guess.
+
+  (*
+   * Swap call to PMS_KEM.enc with A.choose in main, so as to be able
+   * to abort when the challenge pms is queried to extract.
+   * In addition, inline definition of MS_KEM.dec in dec oracle, and 
+   * replace the call to PMS_KEM.dec with its functional spec decrypt.
+   *)
   local module RCCA0 = {
     module O = {
       fun dec(p:version * hash, t:label, c:ciphertext) : ms option = {
         var pv : version;
         var h : hash;
         var pms : pms;
+        var maybe_pms : pms option;
         var k : ms;
         var maybe_k : ms option = None;
         if (!mem t W.labels /\ mem p P) { 
           W.labels = add t W.labels;
           (pv, h) = p;
-          pms = decrypt W.sk pv c;
-          k = RO_KEF.extract(h, (pms, t));
-          maybe_k = if (!mem k W.keys) then Some k else None;
+          maybe_pms = decrypt pv W.sk c;
+          pms = $dpms pv;
+          pms = if maybe_pms = None then pms else proj maybe_pms;
+          k = RO_KEF.extract((pv, h), (pms, t));
+          maybe_k = if (W.guess => !mem k W.keys \/ t <> W.t) 
+                    then Some k else None;
         }
         return maybe_k;
       }
@@ -382,7 +402,6 @@ section.
       var b, b', valid : bool;
       var k0, k1 : ms;
       var c : ciphertext;
-      var t : label;
       var pk : pkey;
       var pv : version;
       var pms : pms;
@@ -391,14 +410,17 @@ section.
       (pk, W.sk) = MS_KEM.keygen();
       W.keys = FSet.empty;
       W.labels = FSet.empty;
+      W.t = pick FSet.empty;
+      W.guess = false;
       (pv, h) = pp;
-      (pms, c) = PMS_KEM.enc((), pk, pv);
-      t = A.choose(pk);
-      valid = !mem t W.labels;
-      k0 = RO_KEF.extract(h, (pms, t));
+      (pms, c) = PMS_KEM.enc(pv, pk, ());
+      W.t = A.choose(pk);
+      valid = !mem W.t W.labels;
+      k0 = RO_KEF.extract((pv, h), (pms, W.t));
       k1 = $key;
       b = ${0,1};
       W.keys = add k0 (add k1 W.keys);
+      W.guess = true;
       b' = A.guess(c, if b then k1 else k0);
       return (b = b' /\ valid);
     }
@@ -410,24 +432,28 @@ section.
     ={res} /\ ={glob W, glob RO_KEF}.
   proof.
     fun; sp; if => //.
-    inline KEM(RO_KEF, PMS_KEM).dec; wp; sp.
-    call (_: ={glob W, glob RO_KEF}); first by eqobs_in.
-    exists * sk{1}, pv{1}, c0{1}; elim *; intros sk pv c.
-    by call{1} (dec_spec sk pv c). 
+    inline KEM(RO_KEF, PMS_KEM).dec; sp.
+    seq 1 0 : (={maybe_k, maybe_pms, pv, h, p, t, c, glob W, glob RO_KEF} /\ 
+      maybe_k{1} = None /\
+      (maybe_pms = decrypt pv W.sk c){2} /\ (t0 = t){1}).
+      exists * sk{1}, pv{1}, c0{1}; elim *; intros sk pv c.
+      by call{1} (dec_spec sk pv c).
+    wp; call (_: ={glob W, glob RO_KEF}); first by eqobs_in.
+    by wp; rnd; skip; progress; smt.
   qed.    
-   
+
   local equiv RCCA_RCCA0 : 
     RCCA(MS_KEM, A(RO_KEF)).main ~ RCCA0.main : true ==> ={res}.
   proof.
     fun.
-    swap{2} [5..6] 1.
+    swap{2} 9 -2.
     call (_: ={glob W, glob RO_KEF}).
       by apply RCCA_RCCA0_dec.
       by fun; eqobs_in.
     inline KEM(RO_KEF, PMS_KEM).enc.
     wp; rnd; rnd; wp.
     call (_: ={glob W, glob RO_KEF}); first by eqobs_in.
-    seq 5 5 : (={t, pk, glob A, glob W, glob RO_KEF} /\ keypair(pk, W.sk){1}).
+    seq 7 7 : (={pk, glob A, glob W, glob RO_KEF} /\ keypair(pk, W.sk){1}).
     call (_: ={glob W, glob RO_KEF}).
       by apply RCCA_RCCA0_dec.
       by fun; eqobs_in.
@@ -438,7 +464,624 @@ section.
     by wp; call (enc_spec_rel sk pk pv); skip; progress; smt.
   qed.
 
-  (* Global variables in RCCA1 and RCCA2 *)
+
+  (* Distinguisher for transformation from lazy to eagerly sampled fake pms's *)
+  local module D(Fake:LE.Types.ARO) : LE.Types.Dist(Fake) = {
+    var m : ((version* hash) * (pms * label), ms) map
+
+    module O1 = {
+      fun extract(p:version * hash, s:pms * label) : ms = {
+        var pms : pms;
+        var t : label;
+        (pms, t) = s;
+        if (!in_dom (p, (pms, t)) m) m.[(p, (pms, t))] = $key;
+        return proj m.[(p, (pms, t))];
+      }
+    }
+
+    module O2 = {
+      fun dec(p:version * hash, t:label, c:ciphertext) : ms option = {
+        var pv : version;
+        var h : hash;
+        var pms : pms;
+        var maybe_pms : pms option;
+        var k : ms;
+        var maybe_k : ms option = None;
+        if (!mem t W.labels /\ mem p P) { 
+          W.labels = add t W.labels;
+          (pv, h) = p;
+          maybe_pms = decrypt pv W.sk c;
+          if (maybe_pms = None) {
+            pms = Fake.o((pv, t));
+            k = O1.extract((pv, h), (pms, t));
+          }
+          else k = O1.extract((pv, h), (proj maybe_pms, t));
+          maybe_k = if (W.guess => !mem k W.keys \/ t <> W.t) 
+                    then Some k else None;
+        }
+        return maybe_k;
+      }
+    }
+
+    module A = A(O1, O2)
+
+    fun distinguish() : bool = {
+      var b, b', valid : bool;
+      var k0, k1 : ms;
+      var c : ciphertext;
+      var pk : pkey;
+      var pv : version;
+      var pms : pms;
+      var h : hash;
+      PMS_KEM.init();
+      (pk, W.sk) = MS_KEM.keygen();
+      W.keys = FSet.empty;
+      W.labels = FSet.empty;
+      W.t = pick FSet.empty;
+      W.guess = false;
+      m = Core.empty;
+      (pv, h) = pp;
+      (pms, c) = PMS_KEM.enc(pv, pk, ());
+      W.t = A.choose(pk);
+      valid = !mem W.t W.labels;
+      k0 = O1.extract((pv, h), (pms, W.t));
+      k1 = $key;
+      b = ${0,1};
+      W.keys = add k0 (add k1 W.keys);
+      W.guess = true;
+      b' = A.guess(c, if b then k1 else k0);
+      return (b = b' /\ valid);
+    }
+  }.
+
+  (* Here is where the condition !mem t labels in dec is used *)
+  local equiv RCCA0_Lazy : 
+   RCCA0.main ~ LE.Types.IND(LE.Lazy.RO, D).main : true ==> ={res}.
+  proof.
+    fun.
+    inline LE.Types.IND(LE.Lazy.RO, D).D.distinguish
+           MS_KEM.init MS_KEM.keygen RO_KEF.init; wp.
+    call (_: 
+      ={glob W} /\ RO_KEF.m{1} = D.m{2} /\
+      (forall t, in_dom t LE.Lazy.RO.m => mem (snd t) W.labels){2}).
+    fun.
+      sp; if => //; sp; if{2}; wp.
+      call (_: 
+        ={glob W} /\ RO_KEF.m{1} = D.m{2} /\
+        (forall t, in_dom t LE.Lazy.RO.m => mem (snd t) W.labels){2}).
+      by sp; if => //; try rnd.
+      by inline LE.Lazy.RO.o; wp; sp; rnd; skip; progress; smt.
+      call (_: 
+        ={glob W} /\ RO_KEF.m{1} = D.m{2} /\
+        (forall t, in_dom t LE.Lazy.RO.m => mem (snd t) W.labels){2}).
+      by sp; if => //; try rnd.
+      by wp; rnd{1}; skip; progress; smt.
+    by fun; sp; if => //; try rnd.
+    wp; rnd; rnd.
+    call (_: 
+      ={glob W} /\ RO_KEF.m{1} = D.m{2} /\
+      (forall t, in_dom t LE.Lazy.RO.m => mem (snd t) W.labels){2}).
+    by sp; if => //; try rnd.
+    wp.
+    call (_: 
+      ={glob W} /\ RO_KEF.m{1} = D.m{2} /\
+      (forall t, in_dom t LE.Lazy.RO.m => mem (snd t) W.labels){2}).
+    fun.
+      sp; if => //; sp; if{2}; wp.
+      call (_: 
+        ={glob W} /\ RO_KEF.m{1} = D.m{2} /\
+        (forall t, in_dom t LE.Lazy.RO.m => mem (snd t) W.labels){2}).
+      by sp; if => //; try rnd.
+      by inline LE.Lazy.RO.o; wp; sp; rnd; skip; progress; smt.
+      call (_: 
+        ={glob W} /\ RO_KEF.m{1} = D.m{2} /\
+        (forall t, in_dom t LE.Lazy.RO.m => mem (snd t) W.labels){2}).
+      by sp; if => //; try rnd.
+      by wp; rnd{1}; skip; progress; smt.
+    by fun; sp; if => //; try rnd.
+    wp; call (_: true); wp; call (_: true); wp; call (_: true); wp.
+    by inline LE.Lazy.RO.init; wp; skip; progress; smt.
+  qed.
+
+
+  (* Eager version of RCCA0 *)
+  local module RCCA1 = {
+    var m : ((version * hash) * (pms * label), ms) map
+    var fake : (version * label, pms) map
+
+    module O1 = {
+      fun extract(p:version * hash, s:pms * label) : ms = {
+        var pms : pms;
+        var t : label;
+        (pms, t) = s;
+        if (!in_dom (p, (pms, t)) m) m.[(p, (pms, t))] = $key;
+        return proj m.[(p, (pms, t))];
+      }
+    }
+
+    module O2 = {
+      fun dec(p:version * hash, t:label, c:ciphertext) : ms option = {
+        var pv : version;
+        var h : hash;
+        var pms : pms;
+        var maybe_pms : pms option;
+        var k : ms;
+        var maybe_k : ms option = None;
+        if (!mem t W.labels /\ mem p P) { 
+          W.labels = add t W.labels;
+          (pv, h) = p;
+          maybe_pms = decrypt pv W.sk c;
+          if (maybe_pms = None) {
+            pms = proj fake.[(pv, t)];
+            k = O1.extract((pv, h), (pms, t));
+          }
+          else k = O1.extract((pv, h), (proj maybe_pms, t));
+          maybe_k = if (W.guess => !mem k W.keys \/ t <> W.t) 
+                    then Some k else None;
+        }
+        return maybe_k;
+      }
+    }
+
+    module A = A(O1, O2)
+
+    fun sample() : unit = {
+      var t : version * label;
+      var labels = toFSet univ;
+      fake = Core.empty;
+      while (labels <> FSet.empty) {
+        t = pick labels;
+        fake.[t] = $dpms (fst t);
+        labels = rm t labels;
+      }
+    }
+
+    fun main() : bool = {
+      var b, b', valid : bool;
+      var k0, k1 : ms;
+      var c : ciphertext;
+      var pk : pkey;
+      var pv : version;
+      var pms : pms;
+      var h : hash;
+      sample();
+      PMS_KEM.init();
+      (pk, W.sk) = MS_KEM.keygen();
+      W.keys = FSet.empty;
+      W.labels = FSet.empty;
+      W.t = pick FSet.empty;
+      W.guess = false;
+      m = Core.empty;
+      (pv, h) = pp;
+      (pms, c) = PMS_KEM.enc(pv, pk, ());
+      W.t = A.choose(pk);
+      valid = !mem W.t W.labels;
+      k0 = O1.extract((pv, h), (pms, W.t));
+      k1 = $key;
+      b = ${0,1};
+      W.keys = add k0 (add k1 W.keys);
+      W.guess = true;
+      b' = A.guess(c, if b then k1 else k0);
+      return (b = b' /\ valid);
+    }
+  }.
+
+  local equiv Eager_RCCA1 : 
+    LE.Types.IND(LE.Eager.RO, D).main ~ RCCA1.main : true ==> ={res}.
+  proof.
+    fun.
+    inline LE.Types.IND(LE.Eager.RO, D).D.distinguish
+           MS_KEM.init MS_KEM.keygen RO_KEF.init; wp.
+    call (_: 
+      ={glob W} /\ D.m{1} = RCCA1.m{2} /\ LE.Eager.RO.m{1} = RCCA1.fake{2}).
+    fun.
+      sp; if => //; sp; if => //; wp.
+      call (_: 
+        ={glob W} /\ D.m{1} = RCCA1.m{2} /\ LE.Eager.RO.m{1} = RCCA1.fake{2}).
+      by sp; if => //; try rnd.
+      by inline LE.Eager.RO.o; wp.
+      call (_: 
+        ={glob W} /\ D.m{1} = RCCA1.m{2} /\ LE.Eager.RO.m{1} = RCCA1.fake{2}) => //.
+      by sp; if => //; try rnd.
+    by fun; sp; if => //; try rnd.
+    wp; rnd; rnd.
+    call (_: 
+      ={glob W} /\ D.m{1} = RCCA1.m{2} /\ LE.Eager.RO.m{1} = RCCA1.fake{2}).
+    by sp; if => //; try rnd.
+    wp.
+    call (_: 
+      ={glob W} /\ D.m{1} = RCCA1.m{2} /\ LE.Eager.RO.m{1} = RCCA1.fake{2}).
+    fun.
+      sp; if => //; sp; if => //; wp.
+      call (_: 
+        ={glob W} /\ D.m{1} = RCCA1.m{2} /\ LE.Eager.RO.m{1} = RCCA1.fake{2}).
+      by sp; if => //; try rnd.
+      by inline LE.Eager.RO.o; wp.
+      call (_: 
+        ={glob W} /\ D.m{1} = RCCA1.m{2} /\ LE.Eager.RO.m{1} = RCCA1.fake{2}) => //.
+      by sp; if => //; try rnd.
+    by fun; sp; if => //; try rnd.
+    wp; call (_: true); wp; call (_: true); wp; call (_: true); wp.
+    inline LE.Eager.RO.init RCCA1.sample; sp.
+    while (work{1} = labels{2} /\ LE.Eager.RO.m{1} = RCCA1.fake{2}) => //.
+    by wp; sp; rnd.
+  qed.
+
+  local equiv RCCA0_RCCA1 : RCCA0.main ~ RCCA1.main : true ==> ={res}.
+  proof.
+    bypr (res{1}) (res{2}) => //.
+    intros &1 &2 b.
+    apply (eq_trans _ Pr[LE.Types.IND(LE.Lazy.RO, D).main() @ &1: b = res]).
+    by equiv_deno RCCA0_Lazy.
+    apply (eq_trans _ Pr[LE.Types.IND(LE.Eager.RO, D).main() @ &1: b = res]).
+    equiv_deno (LE.eagerRO D _) => //; first by smt.
+    by equiv_deno Eager_RCCA1.
+  qed.
+
+  local lemma Pr_RCCA0_RCCA1 &m :
+    Pr[RCCA0.main() @ &m : res] = Pr[RCCA1.main() @ &m : res].
+  proof.
+    by equiv_deno RCCA0_RCCA1.
+  qed.
+
+
+  (* 
+   * Similar to RCCA1, but the decryption oracle does not query extract when
+   * given an invalid ciphertext (i.e. with a randomly generated fake pms)
+   *
+   * This only makes a difference if the adversary queries extract directly
+   * with one of the fake pms's generated internally during decryption in RCCA1.
+   *
+   *)
+  local module RCCA2 = {
+    var m : ((version * hash) * (pms * label), ms) map
+    var fake : (version * label, pms) map
+
+    module O1 = {
+      fun extract(p:version * hash, s:pms * label) : ms = {
+        var pms : pms;
+        var t : label;
+        (pms, t) = s;
+        if (!in_dom (p, (pms, t)) m) m.[(p, (pms, t))] = $key;
+        return proj m.[(p, (pms, t))];
+      }
+    }
+
+    module O2 = {
+      fun dec(p:version * hash, t:label, c:ciphertext) : ms option = {
+        var pv : version;
+        var h : hash;
+        var pms : pms;
+        var maybe_pms : pms option;
+        var k : ms;
+        var maybe_k : ms option = None;
+        if (!mem t W.labels /\ mem p P) { 
+          W.labels = add t W.labels;
+          (pv, h) = p;
+          maybe_pms = decrypt pv W.sk c;
+          if (maybe_pms = None) k = $key;
+          else k = O1.extract((pv, h), (proj maybe_pms, t));
+          maybe_k = if (W.guess => !mem k W.keys \/ t <> W.t) 
+                    then Some k else None;
+        }
+        return maybe_k;
+      }
+    }
+
+    module A = A(O1, O2)
+
+    fun sample() : unit = {
+      var t : version * label;
+      var labels = toFSet univ;
+      fake = Core.empty;
+      while (labels <> FSet.empty) {
+        t = pick labels;
+        fake.[t] = $dpms (fst t);
+        labels = rm t labels;
+      }
+    }
+
+    fun main() : bool = {
+      var b, b', valid : bool;
+      var k0, k1 : ms;
+      var c : ciphertext;
+      var pk : pkey;
+      var pv : version;
+      var pms : pms;
+      var h : hash;
+      sample();
+      PMS_KEM.init();
+      (pk, W.sk) = MS_KEM.keygen();
+      W.keys = FSet.empty;
+      W.labels = FSet.empty;
+      W.t = pick FSet.empty;
+      W.guess = false;
+      m = Core.empty;
+      (pv, h) = pp;
+      (pms, c) = PMS_KEM.enc(pv, pk, ());
+      W.t = A.choose(pk);
+      valid = !mem W.t W.labels;
+      k0 = O1.extract((pv, h), (pms, W.t));
+      k1 = $key;
+      b = ${0,1};
+      W.keys = add k0 (add k1 W.keys);
+      W.guess = true;
+      b' = A.guess(c, if b then k1 else k0);
+      return (b = b' /\ valid);
+    }
+  }.
+
+  local equiv RCCA1_RCCA2_extract :
+    RCCA1.O1.extract ~ RCCA2.O1.extract : 
+    !(exists pv h t, in_dom ((pv, h), (proj RCCA2.fake.[(pv, t)], t)) RCCA2.m){2} /\
+    ={p, s} /\ ={glob W} /\ RCCA1.fake{1} = RCCA2.fake{2} /\
+    (forall p, in_dom p RCCA1.fake){1} /\
+    (forall pv h t, 
+     in_dom ((pv, h), (proj RCCA1.fake.[(pv, t)], t)) RCCA1.m => mem t W.labels){1} /\
+    forall pv h pms t, pms <> proj RCCA1.fake{1}.[(pv, t)] => 
+      RCCA1.m{1}.[((pv, h), (pms, t))] = RCCA2.m{2}.[((pv, h), (pms, t))]
+    ==>
+   !(exists pv h t, in_dom ((pv, h), (proj RCCA2.fake.[(pv, t)], t)) RCCA2.m){2} =>
+      ={res} /\ ={glob W} /\ RCCA1.fake{1} = RCCA2.fake{2} /\
+      (forall p, in_dom p RCCA1.fake){1} /\
+      (forall pv h t, 
+       in_dom ((pv, h), (proj RCCA1.fake.[(pv, t)], t)) RCCA1.m => mem t W.labels){1} /\
+      forall pv h pms t, pms <> proj RCCA1.fake{1}.[(pv, t)] => 
+        RCCA1.m{1}.[((pv, h), (pms, t))] = RCCA2.m{2}.[((pv, h), (pms, t))].
+  proof.  
+    fun; sp.
+    case (pms = proj RCCA2.fake.[(fst p, t)]){2}.
+      (* pms = proj RCCA2.fake[t] *)
+      if{1}; if{2}.
+        rnd; skip; progress.
+          by smt.
+          by smt.
+          by rewrite /_.[_] Core.get_setN; smt.
+        rnd{1}; skip; progress.
+          by smt.
+          cut X : exists pv h t,
+            in_dom ((pv, h), (proj RCCA2.fake{2}.[(pv, t)], t)) RCCA2.m{2}.
+            by exists (fst p{2}), (snd p{2}), t{2}; smt.
+            by smt.
+          by smt.
+          by smt.
+        rnd{2}; skip; progress.
+          by smt.
+          cut X : exists pv h t,
+            in_dom ((pv, h), (proj RCCA2.fake{2}.[(pv, t)], t)) RCCA2.m{2}.
+            by exists (fst p{2}), (snd p{2}), t{2}; smt.
+            by smt.
+          by smt.
+       skip; progress.
+       cut X : exists pv h t,
+         in_dom ((pv, h), (proj RCCA2.fake{2}.[(pv, t)], t)) RCCA2.m{2}.
+         by exists (fst p{2}), (snd p{2}), t{2}; smt.
+         by smt.
+      (* pms <> proj RCCA2.fake[t] *)
+      if => //.
+        progress.
+        by cut X := H2 (fst p{2}) (snd p{2}) pms{2} t{2}; smt.
+        by cut X := H2 (fst p{2}) (snd p{2}) pms{2} t{2}; smt.
+        rnd; skip; progress.
+          by smt.
+          by smt.
+          by case ((p, (pms, t)){2} = ((pv, h), (pms0, t0))); smt.
+        skip; progress.
+        by cut X := H2 (fst p{2}) (snd p{2}) pms{2} t{2}; smt.
+  qed.
+
+  local equiv RCCA1_RCCA2_dec :
+    RCCA1.O2.dec ~  RCCA2.O2.dec :
+    !(exists pv h t, in_dom ((pv, h), (proj RCCA2.fake.[(pv, t)], t)) RCCA2.m){2} /\
+    ={p, t, c} /\ ={glob W} /\ RCCA1.fake{1} = RCCA2.fake{2} /\
+    (forall p, in_dom p RCCA1.fake){1} /\
+    (forall pv h t, 
+     in_dom ((pv, h), (proj RCCA1.fake.[(pv, t)], t)) RCCA1.m => mem t W.labels){1} /\
+    forall pv h pms t, pms <> proj RCCA1.fake{1}.[(pv, t)] => 
+      RCCA1.m{1}.[((pv, h), (pms, t))] = RCCA2.m{2}.[((pv, h), (pms, t))]
+    ==>
+    !(exists pv h t, in_dom ((pv, h), (proj RCCA2.fake.[(pv, t)], t)) RCCA2.m){2} =>
+      ={res} /\ ={glob W} /\ RCCA1.fake{1} = RCCA2.fake{2} /\
+      (forall p, in_dom p RCCA1.fake){1} /\
+      (forall pv h t, 
+       in_dom ((pv, h), (proj RCCA1.fake.[(pv, t)], t)) RCCA1.m => mem t W.labels){1} /\
+      forall pv h pms t, pms <> proj RCCA1.fake{1}.[(pv, t)] => 
+        RCCA1.m{1}.[((pv, h), (pms, t))] = RCCA2.m{2}.[((pv, h), (pms, t))].
+  proof.  
+    fun; sp; if => //.
+      sp; if => //.
+        inline RCCA1.O1.extract; wp; sp.
+        if{1}.
+          by rnd; skip; progress; smt.
+          by rnd{2}; skip; progress; smt.
+      wp; call RCCA1_RCCA2_extract.
+      by skip; progress; smt.
+  qed.
+
+  local equiv RCCA1_RCCA2 :
+    RCCA1.main ~ RCCA2.main : 
+    true ==>  
+    !(exists pv h t, in_dom ((pv, h), (proj RCCA2.fake.[(pv, t)], t)) RCCA2.m){2} => ={res}.
+  proof.
+    fun.
+    seq 12 12 :
+      (!(exists pv h t, in_dom ((pv, h), (proj RCCA2.fake.[(pv, t)], t)) RCCA2.m){2} =>
+      ={glob W, glob A, pk, pv, h, pms, c, valid} /\ 
+      RCCA1.fake{1} = RCCA2.fake{2} /\
+      (forall p, in_dom p RCCA1.fake){1} /\
+      (forall pv h t, 
+        in_dom ((pv, h), (proj RCCA1.fake.[(pv, t)], t)) RCCA1.m => mem t W.labels){1} /\
+      forall pv h pms t, pms <> proj RCCA1.fake{1}.[(pv, t)] => 
+        RCCA1.m{1}.[((pv, h), (pms, t))] = RCCA2.m{2}.[((pv, h), (pms, t))]).
+    wp; call (_:
+     (exists pv h t, in_dom ((pv, h), (proj RCCA2.fake.[(pv, t)], t)) RCCA2.m),
+     ={glob W} /\ RCCA1.fake{1} = RCCA2.fake{2} /\
+     (forall p, in_dom p RCCA1.fake){1} /\
+     (forall pv h t, 
+       in_dom ((pv, h), (proj RCCA1.fake.[(pv, t)], t)) RCCA1.m => mem t W.labels){1} /\
+     forall pv h pms t, pms <> proj RCCA1.fake{1}.[(pv, t)] => 
+       RCCA1.m{1}.[((pv, h), (pms, t))] = RCCA2.m{2}.[((pv, h), (pms, t))]).
+     by apply lossless_choose.
+     by apply RCCA1_RCCA2_dec.
+     intros &2 ?; fun; sp; if => //.
+     wp; sp; inline RCCA1.O1.extract; if.
+       by wp; sp; if => //; rnd; skip; smt.
+       by wp; sp; if => //; rnd; skip; smt.
+     intros &1; fun.
+     sp; if; wp; sp => //.
+     if.  
+       by rnd; skip; progress; smt.
+       inline RCCA2.O1.extract; wp; sp; if => //.
+       by rnd Fun.cpTrue; skip; progress; smt.
+     by apply RCCA1_RCCA2_extract.
+     by progress; fun; wp; sp; if; try rnd; skip; smt.
+     by intros _; fun; sp; if => //; rnd Fun.cpTrue; skip; progress; smt.
+
+     wp; call (_: ={glob W} /\ RCCA1.fake{1} = RCCA2.fake{2}); wp.
+     call (_:RCCA1.fake{1} = RCCA2.fake{2}).
+     eqobs_in; progress; apply stateless_pms_kem.
+     call (_:true); wp.
+     call (_:true ==> RCCA1.fake{1} = RCCA2.fake{2} /\
+                      forall p, (in_dom p RCCA1.fake){1}).
+     fun; sp.
+     while (={labels} /\ RCCA1.fake{1} = RCCA2.fake{2} /\
+            forall p, (!mem p labels => in_dom p RCCA1.fake){1}).
+     by wp; rnd; wp; skip; progress; smt.
+     by wp; skip; progress; smt.
+     by wp; skip; progress; smt.
+
+     case ((proj RCCA2.fake.[(pv, W.t)] = pms){2} \/
+           exists pv h t, in_dom ((pv, h), (proj RCCA2.fake.[(pv, t)], t)) RCCA2.m){2}.
+     seq 1 1 : (exists pv h t, in_dom ((pv, h), (proj RCCA2.fake.[(pv, t)], t)) RCCA2.m){2}.
+     inline RCCA1.O1.extract RCCA2.O1.extract; wp; sp.      
+     if{1}; if{2}.
+       rnd; skip; progress; elim H0 => ?.
+         by exists pv{2}, h{2}, W.t{2}; smt.
+         by smt.
+       by rnd{1}; skip; progress; smt.
+       rnd{2}; skip; progress; [smt | elim H0 => ?].
+         by exists pv{2}, h{2}, W.t{2}; smt.
+         by smt.
+       by skip; progress; smt.
+     call (_:true, true,
+      (exists pv h t, in_dom ((pv, h), (proj RCCA2.fake.[(pv, t)], t)) RCCA2.m){2}).
+        by apply lossless_guess.
+        by exfalso; smt.
+        (* by apply RCCA1_dec_preserves_bad. *)
+        progress; fun; sp; if => //.
+        wp; sp; inline RCCA1.O1.extract; if.
+          by wp; sp; if => //; rnd; skip; smt.
+          by wp; sp; if => //; rnd; skip; smt.
+        (* by apply RCCA2_dec_preserves_bad. *)
+        progress; fun; sp; if => //.
+        wp; sp; inline RCCA1.O1.extract; if.
+          by rnd; skip; progress; smt.
+          inline RCCA2.O1.extract; wp; sp; if => //.
+          by rnd Fun.cpTrue; skip; progress; smt.
+        by exfalso; smt.
+        (* by apply RCCA1_extract_preserves_bad. *)
+        by progress; fun; wp; sp; if; try rnd; skip; smt.
+        (* by apply RCCA2_extract_preserves_bad. *)
+        by progress; fun; sp; if => //; rnd Fun.cpTrue; skip; smt.
+     wp; rnd; rnd; inline RCCA1.O1.extract RCCA2.O1.extract; wp; sp.      
+     by skip; progress; smt. 
+
+    call (_:
+     (exists pv h t, in_dom ((pv, h), (proj RCCA2.fake.[(pv, t)], t)) RCCA2.m),
+     ={glob W} /\ RCCA1.fake{1} = RCCA2.fake{2} /\
+     (forall t, in_dom t RCCA1.fake){1} /\
+     (forall pv h t, 
+       in_dom ((pv, h), (proj RCCA1.fake.[(pv, t)], t)) RCCA1.m => mem t W.labels){1} /\
+     forall pv h pms t, pms <> proj RCCA1.fake{1}.[(pv, t)] => 
+       RCCA1.m{1}.[((pv, h), (pms, t))] = RCCA2.m{2}.[((pv, h), (pms, t))]).
+     by apply lossless_guess.
+     by apply RCCA1_RCCA2_dec.
+     progress; fun; sp; if => //.
+     wp; sp; inline RCCA1.O1.extract; if.
+       by wp; sp; if => //; rnd; skip; smt.
+       by wp; sp; if => //; rnd; skip; smt.
+     intros &1; fun.
+     sp; if; wp; sp => //.
+     if.  
+       by rnd ; skip; progress; smt.
+       inline RCCA2.O1.extract; wp; sp; if => //.
+       by rnd Fun.cpTrue; skip; progress; smt.
+     by apply RCCA1_RCCA2_extract.
+     by progress; fun; wp; sp; if; try rnd; skip; smt.
+     by progress; fun; sp; if => //; rnd Fun.cpTrue; skip; progress; smt.
+    
+     wp; rnd; rnd.
+     inline RCCA1.O1.extract RCCA2.O1.extract; wp; sp.      
+     if => //.
+       intros ? ? ?.
+       cut X : !(exists pv h t, 
+         in_dom ((pv, h), (proj RCCA2.fake{2}.[(pv, t)], t)) RCCA2.m{2}) by smt.
+         generalize H; rewrite X => /=; progress; smt. 
+
+       rnd; skip; progress; [smt | smt | smt | smt | smt | smt | smt | smt | smt | | | ].
+         cut X : !(exists pv h t, in_dom 
+           ((pv, h), (proj RCCA2.fake{2}.[(pv, t)], t)) RCCA2.m{2}) by smt.
+         generalize H; rewrite X => /=; progress.
+         by smt.
+         cut X : !(exists pv h t, in_dom 
+           ((pv, h), (proj RCCA2.fake{2}.[(pv, t)], t)) RCCA2.m{2}) by smt.
+         generalize H; rewrite X => /=; progress.
+         case (((pv0, h0), (pms1, t0)) = ((pv, h), (pms, W.t)){2}) => ?; first by smt.
+         by cut V := H14 pv0 h0 pms1 t0; smt.
+         cut X : !(exists pv h t, in_dom 
+           ((pv, h), (proj RCCA2.fake{2}.[(pv, t)], t)) RCCA2.m{2}) by smt.
+         generalize H; rewrite X => /=; progress.
+         by smt.
+      skip; progress; [smt | smt | smt | smt | smt | smt | smt | smt | smt | smt | smt | ].          
+      cut X : !(exists pv h t, in_dom 
+        ((pv, h), (proj RCCA2.fake{2}.[(pv, t)], t)) RCCA2.m{2}) by smt.
+        generalize H; rewrite X => /=; progress.
+        generalize H9; rewrite H10 => /=; progress.
+  qed. 
+
+  local lemma Pr_RCCA1_RCCA2 &m :
+    Pr[RCCA1.main() @ &m : res] <=
+    Pr[RCCA2.main() @ &m : res] +
+    Pr[RCCA2.main() @ &m : exists pv h t, in_dom ((pv, h), (proj RCCA2.fake.[(pv, t)], t)) RCCA2.m].
+  proof.
+    apply (Trans _ 
+     Pr[RCCA2.main() @ &m : res \/ 
+      exists pv h t, in_dom ((pv, h), (proj RCCA2.fake.[(pv, t)], t)) RCCA2.m]).
+    by equiv_deno RCCA1_RCCA2; smt.  
+    by rewrite Pr mu_or; smt.    
+  qed.
+
+
+  (* Maximum number of queries to KEF extract oracle *)
+  const qKEF : int.
+
+  axiom qKEF_pos : 0 < qKEF.
+
+  (* Assuming that fake pms's are uniformly random to have a readable bound *)
+  axiom dpms_uniform pms : forall pv,
+    Distr.mu_x (dpms pv) pms = 1%r / (card (toFSet univ<:pms>))%r.
+
+  local lemma Pr_RCCA2 &m :
+    Pr[RCCA2.main() @ &m : exists pv h t, in_dom ((pv, h), (proj RCCA2.fake.[(pv, t)], t)) RCCA2.m] <=
+    qKEF%r / (card (toFSet univ<:pms>))%r.
+  proof.
+    bdhoare_deno 
+      (_:true ==> exists pv h t, in_dom ((pv, h), (proj RCCA2.fake.[(pv, t)], t)) RCCA2.m) => //;
+    last by smt.
+    fun; swap 14; inline RCCA2.sample.
+    (*
+     * dom(m) = { (pv_1, h_1, pms_1, t_1), ..., (h_q, pms_q, t_q) }
+     * q <= q_DEC + q_KEF
+     * 
+     * Pr[exists pv h t, (pv, h, fake[pv, t], t) in dom(m)] <= 
+     * sum_{pv \in version, t \in labels} sum_{i=1..q} 
+     *   Pr[fake[pv, t] = pms_i /\ pv = pv_i /\ t = t_i] <=
+     * sum_{i=1..q} Pr[fake[pv_i, t_i] = pms_i] = q / |pms|
+     *)
+    admit.
+  qed.
+
+  (* Global variables in RCCA3 and RCCA4 *)
   local module V = {
     var pk : pkey
     var sk : skey
@@ -458,17 +1101,23 @@ section.
       pms = pick FSet.empty;
     }
   }.
-  
-  local module RCCA1 = {
-    var m : (hash * (pms * label), ms) map
+
+  (*
+   * This game "aborts" when the simulation fails, but still uses the PMS KEM
+   * secret key to detect when to abort and implement the simulation.
+   * However, all uses of the secret key for simulation could be implemented
+   * using a plaintext-checking oracle instead.
+   *)
+  local module RCCA3 = {
+    var m : ((version * hash) * (pms * label), ms) map
     var abort : bool
   
     module O1 = {
-      fun extract(p:hash, s:pms * label) : ms = {
+      fun extract(p:version * hash, s:pms * label) : ms = {
         var pms : pms;
         var t : label;
         (pms, t) = s;
-        abort = abort \/ (p = snd pp /\ pms = V.pms);
+        abort = abort \/ (p = pp /\ pms = V.pms);
         if (!in_dom (p, (pms, t)) m) m.[(p, (pms, t))] = $key;
         return proj m.[(p, (pms, t))];
       }
@@ -479,17 +1128,24 @@ section.
         var pv : version;
         var h : hash;
         var pms : pms;
+        var maybe_pms : pms option;
         var k : ms;
         var maybe_k : ms option = None;
         if (!mem t V.labels /\ mem p P) { 
           V.labels = add t V.labels;
           (pv, h) = p;
-          pms = decrypt V.sk pv c;
-          abort = abort \/ (V.guess /\ pms = V.pms /\ t = V.t /\ c <> V.c);
-          if (!(V.guess /\ same_key V.pk (fst pp) pv c /\ h = snd pp /\ t = V.t /\ c = V.c)) {
-            if (!in_dom (h, (pms, t)) m) m.[(h, (pms, t))] = $key;
-            k = proj m.[(h, (pms, t))];
-            maybe_k = if (!mem k V.keys) then Some k else None;
+          maybe_pms = decrypt pv V.sk c;
+          abort = abort \/ 
+           (V.guess /\ maybe_pms <> None /\ proj maybe_pms = V.pms /\ p = pp /\ t = V.t /\ c <> V.c);
+          if (!(V.guess /\ p = pp /\ t = V.t /\ c = V.c)) {
+            if (maybe_pms = None) k = $key;
+            else {
+              pms = proj maybe_pms;
+              if (!in_dom ((pv, h), (pms, t)) m) m.[((pv, h), (pms, t))] = $key;
+              k = proj m.[((pv, h), (pms, t))];
+            }
+            maybe_k = if (V.guess => !mem k V.keys \/ t <> V.t) 
+                      then Some k else None;
           }
         }
         return maybe_k;
@@ -506,7 +1162,7 @@ section.
      V.init();
      m = Core.empty;
      abort = false;
-     (V.pms, V.c) = PMS_KEM.enc((), V.pk, fst pp);
+     (V.pms, V.c) = PMS_KEM.enc(fst pp, V.pk, ());
      V.t = A.choose(V.pk);
      valid = !mem V.t V.labels;
      k0 = $key;
@@ -519,35 +1175,80 @@ section.
    }
   }.
   
-  (** RCCA0 -> RCCA1 **)
-  local equiv RCCA0_RCCA1_extract_guess :
-    RO_KEF.extract ~ RCCA1.O1.extract :
-    !RCCA1.abort{2} /\
+  (** RCCA2 -> RCCA3 **)
+  local lemma RCCA2_lossless_extract : islossless RCCA2.O1.extract.
+  proof.
+    by fun; sp; if => //; rnd; skip; progress; smt.
+  qed.
+
+  local lemma RCCA2_lossless_dec : islossless RCCA2.O2.dec.
+  proof.
+    fun.
+    sp; if => //.
+    inline KEM(RO_KEF, PMS_KEM).dec; wp; sp.
+    if => //.
+      by rnd; skip; smt.    
+      by call (_:true ==> true) => //; apply RCCA2_lossless_extract.
+  qed.
+
+  local lemma RCCA3_lossless_extract : islossless RCCA3.O1.extract.
+  proof.
+    by fun; sp; if => //; rnd; skip; progress; smt.
+  qed.
+
+  local lemma RCCA3_lossless_dec : islossless RCCA3.O2.dec.
+  proof.
+    fun.
+    sp; if => //.
+    sp; if => //.
+    if => //; wp.
+      by rnd; skip; smt.
+      by sp; if; try rnd; skip; smt.
+  qed.
+
+  local lemma RCCA3_dec_preserves_abort : 
+    bd_hoare [ RCCA3.O2.dec : RCCA3.abort ==> RCCA3.abort ] = 1%r.
+  proof.
+    fun.
+    sp; if => //.
+    sp; if => //.
+    if => //.
+      by wp; rnd; skip; smt.  
+    sp; if => //; wp; try rnd; skip; smt.
+  qed.
+
+  local equiv RCCA2_RCCA3_extract_guess :
+    RCCA2.O1.extract ~ RCCA3.O1.extract :
+    !RCCA3.abort{2} /\
     ={p, s} /\
     keypair(V.pk, V.sk){2} /\
     V.guess{2} /\
     W.sk{1} = V.sk{2} /\
     W.keys{1} = V.keys{2} /\
     W.labels{1} = V.labels{2} /\
-    eq_except RO_KEF.m{1} RCCA1.m{2} (snd pp, (V.pms, V.t)){2} /\
-    in_dom (snd pp, (V.pms, V.t)){2} RO_KEF.m{1} /\
-    mem (proj RO_KEF.m{1}.[(snd pp, (V.pms, V.t))]){2} V.keys{2} /\
-    decrypt V.sk{2} (fst pp) V.c{2} = V.pms{2}
+    W.t{1} = V.t{2} /\
+    W.guess{1} = V.guess{2} /\
+    eq_except RCCA2.m{1} RCCA3.m{2} (pp, (V.pms, V.t)){2} /\
+    in_dom (pp, (V.pms, V.t)){2} RCCA2.m{1} /\
+    mem (proj RCCA2.m{1}.[(pp, (V.pms, V.t))]){2} V.keys{2} /\
+    decrypt (fst pp) V.sk{2} V.c{2} = Some V.pms{2}
     ==>
-    !RCCA1.abort{2} =>
+    !RCCA3.abort{2} =>
       ={res} /\
       keypair(V.pk, V.sk){2} /\
       V.guess{2} /\
       W.sk{1} = V.sk{2} /\
       W.keys{1} = V.keys{2} /\
       W.labels{1} = V.labels{2} /\
-      eq_except RO_KEF.m{1} RCCA1.m{2} (snd pp, (V.pms, V.t)){2} /\
-      in_dom (snd pp, (V.pms, V.t)){2} RO_KEF.m{1} /\
-      mem (proj RO_KEF.m{1}.[(snd pp, (V.pms, V.t))]){2} V.keys{2} /\
-      decrypt V.sk{2} (fst pp) V.c{2} = V.pms{2}.
+      W.t{1} = V.t{2} /\
+      W.guess{1} = V.guess{2} /\
+      eq_except RCCA2.m{1} RCCA3.m{2} (pp, (V.pms, V.t)){2} /\
+      in_dom (pp, (V.pms, V.t)){2} RCCA2.m{1} /\
+      mem (proj RCCA2.m{1}.[(pp, (V.pms, V.t))]){2} V.keys{2} /\
+      decrypt (fst pp) V.sk{2} V.c{2} = Some V.pms{2}.
   proof.
     fun.
-    sp; case RCCA1.abort{2}.
+    sp; case RCCA3.abort{2}.
       (* aborts *)
       if{1}; if{2}.
         by rnd; skip; smt.
@@ -557,215 +1258,207 @@ section.
       (* doesn't abort *)
       if; first by smt.
         by wp; rnd; skip; progress; smt.    
-        wp; skip; progress.
-        cut W : 
-         (p, (pms, t)){2} <>
-         (snd pp, (decrypt V.sk (fst pp) V.c, V.t)){2} by smt.
-        by generalize H2; rewrite eq_except_def; smt.
+        by skip; progress; smt.
   qed.
   
-  local equiv RCCA0_RCCA1_dec_guess :
-    RCCA0.O.dec ~ RCCA1.O2.dec :
-    !RCCA1.abort{2} /\
+  local equiv RCCA2_RCCA3_dec_guess :
+    RCCA2.O2.dec ~ RCCA3.O2.dec :
+    !RCCA3.abort{2} /\
     ={p, t, c} /\
     keypair(V.pk, V.sk){2} /\
     V.guess{2} /\
     W.sk{1} = V.sk{2} /\
     W.keys{1} = V.keys{2} /\
     W.labels{1} = V.labels{2} /\
-    eq_except RO_KEF.m{1} RCCA1.m{2} (snd pp, (V.pms, V.t)){2} /\
-    in_dom (snd pp, (V.pms, V.t)){2} RO_KEF.m{1} /\
-    mem (proj RO_KEF.m{1}.[(snd pp, (V.pms, V.t))]){2} V.keys{2} /\
-    decrypt V.sk{2} (fst pp) V.c{2} = V.pms{2}
+    W.t{1} = V.t{2} /\
+    W.guess{1} = V.guess{2} /\
+    eq_except RCCA2.m{1} RCCA3.m{2} (pp, (V.pms, V.t)){2} /\
+    in_dom (pp, (V.pms, V.t)){2} RCCA2.m{1} /\
+    mem (proj RCCA2.m{1}.[(pp, (V.pms, V.t))]){2} V.keys{2} /\
+    decrypt (fst pp) V.sk{2} V.c{2} = Some V.pms{2}
     ==>
-    !RCCA1.abort{2} =>
+    !RCCA3.abort{2} =>
       ={res} /\
       keypair(V.pk, V.sk){2} /\
       V.guess{2} /\
       W.sk{1} = V.sk{2} /\
       W.keys{1} = V.keys{2} /\
       W.labels{1} = V.labels{2} /\
-      eq_except RO_KEF.m{1} RCCA1.m{2} (snd pp, (V.pms, V.t)){2} /\
-      in_dom (snd pp, (V.pms, V.t)){2} RO_KEF.m{1} /\
-      mem (proj RO_KEF.m{1}.[(snd pp, (V.pms, V.t))]){2} V.keys{2} /\
-      decrypt V.sk{2} (fst pp) V.c{2} = V.pms{2}.
+      W.t{1} = V.t{2} /\
+      W.guess{1} = V.guess{2} /\
+      eq_except RCCA2.m{1} RCCA3.m{2} (pp, (V.pms, V.t)){2} /\
+      in_dom (pp, (V.pms, V.t)){2} RCCA2.m{1} /\
+      mem (proj RCCA2.m{1}.[(pp, (V.pms, V.t))]){2} V.keys{2} /\
+      decrypt (fst pp) V.sk{2} V.c{2} = Some V.pms{2}.
   proof.
     fun.
     sp; if => //.
-    wp; sp; case RCCA1.abort{2}.
+    wp; sp; case RCCA3.abort{2}.
       (* aborts *)
-      call{1} (_:true ==> true); first by apply lossless_extract.
       if{2}.
-        if{2}.
-          by wp; rnd{2}; skip; smt.
-          by wp; skip; smt.
-        by skip; smt.    
+       if{1}; if{2}.
+         by wp; rnd; skip; progress; smt.
+         sp; if{2}; wp; try rnd; try rnd{1}; skip; progress; smt.
+   
+         call{1} (_:true ==> true); first by apply RCCA2_lossless_extract.
+         by wp; rnd{2}; skip; smt.
+
+         call{1} (_:true ==> true); first by apply RCCA2_lossless_extract.
+         sp; if{2}; wp; try rnd{2}; skip; progress; smt.
+         
+         if{1}.
+           by rnd{1}; skip; smt.
+           call{1} (_:true ==> true); first by apply RCCA2_lossless_extract.
+           by skip; smt.    
       (* doesn't abort *)
-      inline{1} RO_KEF.extract.
+      inline{1} RCCA2.O1.extract.
       if{2}.
+        if => //; first by wp; rnd; skip; progress.
         wp; sp; if.
-          progress.
           by smt.
-          by cut W := same_key_spec V.pk{2} V.sk{2} (fst pp) pv{2} c{2}; smt.
           by rnd; skip; progress; smt.    
         skip; progress.
-        cut W := same_key_spec V.pk{2} V.sk{2} (fst pp) pv{2} c{2}.
         by generalize H2; rewrite eq_except_def; smt.
-    wp; sp; if{1}.
-      by rnd{1}; skip; progress;
-        cut W := same_key_spec V.pk{2} V.sk{2} (fst pp) pv{2} V.c{2}; smt.
-      by skip; progress;
-        cut W := same_key_spec V.pk{2} V.sk{2} (fst pp) pv{2} V.c{2}; smt.
+
+    if{1}; wp; sp.
+      by exfalso; smt.
+      if{1}.
+        by rnd{1}; skip; progress; smt.
+      by skip; progress; smt.
   qed.
   
-  local lemma RCCA0_lossless_dec : islossless RCCA0.O.dec.
-  proof.
-    fun.
-    sp; if => //.
-    inline KEM(RO_KEF, PMS_KEM).dec; wp; sp.
-    seq 1 : true => //.
-      by call (_:true ==> true) => //; apply lossless_extract.
-  qed.
-
-  local lemma RCCA1_lossless_dec : islossless RCCA1.O2.dec.
-  proof.
-    fun.
-    sp; if => //.
-    sp; if => //.
-    by if => //; wp; try rnd; skip; smt.  
-  qed.
-
-  local lemma RCCA1_dec_preserves_abort : 
-    bd_hoare [ RCCA1.O2.dec : RCCA1.abort ==> RCCA1.abort ] = 1%r.
-  proof.
-    fun.
-    sp; if => //.
-    sp; if => //.
-    by if => //; wp; try rnd; skip; smt.  
-  qed.
-  
-  local equiv RCCA0_RCCA1_extract_choose :
-    RO_KEF.extract ~ RCCA1.O1.extract :
-    !RCCA1.abort{2} /\
+  local equiv RCCA2_RCCA3_extract_choose :
+    RCCA2.O1.extract ~ RCCA3.O1.extract :
+    !RCCA3.abort{2} /\
     ={p, s} /\
     keypair(V.pk, V.sk){2} /\ 
     !V.guess{2} /\
-    RO_KEF.m{1} = RCCA1.m{2} /\
+    RCCA2.m{1} = RCCA3.m{2} /\
     W.sk{1} = V.sk{2} /\
     W.keys{1} = V.keys{2} /\
     W.labels{1} = V.labels{2} /\
-    decrypt V.sk{2} (fst pp) V.c{2} = V.pms{2} /\
+    W.t{1} = V.t{2} /\
+    W.guess{1} = V.guess{2} /\
+    decrypt (fst pp) V.sk{2} V.c{2} = Some V.pms{2} /\
     (forall t,
-     in_dom (snd pp, (V.pms, t)) RCCA1.m => 
-     RCCA1.abort \/ mem t V.labels){2}
+     in_dom (pp, (V.pms, t)) RCCA3.m => 
+     RCCA3.abort \/ mem t V.labels){2}
     ==>
-    !RCCA1.abort{2} =>
+    !RCCA3.abort{2} =>
       ={res} /\ 
       keypair(V.pk, V.sk){2} /\
       !V.guess{2} /\
-      RO_KEF.m{1} = RCCA1.m{2} /\
+      RCCA2.m{1} = RCCA3.m{2} /\
       W.sk{1} = V.sk{2} /\
       W.keys{1} = V.keys{2} /\
       W.labels{1} = V.labels{2} /\
-      decrypt V.sk{2} (fst pp) V.c{2} = V.pms{2} /\
+      W.t{1} = V.t{2} /\
+      W.guess{1} = V.guess{2} /\
+      decrypt (fst pp) V.sk{2} V.c{2} = Some V.pms{2} /\
       (forall t,
-       in_dom (snd pp, (V.pms, t)) RCCA1.m => 
-       RCCA1.abort \/ mem t V.labels){2}.
+       in_dom (pp, (V.pms, t)) RCCA3.m => 
+       RCCA3.abort \/ mem t V.labels){2}.
   proof.
     fun.
-    sp; case RCCA1.abort{2}.
+    sp; case RCCA3.abort{2}.
       by if{1}; if{2}; try rnd{1}; try rnd{2}; skip; smt.
       if => //.
         by rnd; skip; smt. 
         by skip; smt.
   qed.
   
-  local equiv RCCA0_RCCA1_dec_choose :
-    RCCA0.O.dec ~ RCCA1.O2.dec :
-    !RCCA1.abort{2} /\
+  local equiv RCCA2_RCCA3_dec_choose :
+    RCCA2.O2.dec ~ RCCA3.O2.dec :
+    !RCCA3.abort{2} /\
     ={p, t, c} /\ 
     keypair(V.pk, V.sk){2} /\
     !V.guess{2} /\
-    RO_KEF.m{1} = RCCA1.m{2} /\
+    RCCA2.m{1} = RCCA3.m{2} /\
     W.sk{1} = V.sk{2} /\
     W.keys{1} = V.keys{2} /\
     W.labels{1} = V.labels{2} /\
-    (decrypt V.sk (fst pp) V.c = V.pms){2} /\
+    W.t{1} = V.t{2} /\
+    W.guess{1} = V.guess{2} /\
+    (decrypt (fst pp) V.sk  V.c = Some V.pms){2} /\
     (forall t,
-     in_dom (snd pp, (V.pms, t)) RCCA1.m => 
-     RCCA1.abort \/ mem t V.labels){2}
+     in_dom (pp, (V.pms, t)) RCCA3.m => 
+     RCCA3.abort \/ mem t V.labels){2}
     ==>
-    !RCCA1.abort{2} =>
+    !RCCA3.abort{2} =>
       ={res} /\ 
       keypair(V.pk, V.sk){2} /\
       !V.guess{2} /\
-      RO_KEF.m{1} = RCCA1.m{2} /\
+      RCCA2.m{1} = RCCA3.m{2} /\
       W.sk{1} = V.sk{2} /\
       W.keys{1} = V.keys{2} /\
       W.labels{1} = V.labels{2} /\
-      (decrypt V.sk (fst pp) V.c = V.pms){2} /\
+      W.t{1} = V.t{2} /\
+      W.guess{1} = V.guess{2} /\
+      (decrypt (fst pp) V.sk V.c = Some V.pms){2} /\
       (forall t,
-       in_dom (snd pp, (V.pms, t)) RCCA1.m => 
-       RCCA1.abort \/ mem t V.labels){2}.
+       in_dom (pp, (V.pms, t)) RCCA3.m => 
+       RCCA3.abort \/ mem t V.labels){2}.
   proof.
     fun.
     sp; if => //.
-    inline{1} RO_KEF.extract; wp; sp.
-    if{2}.
-      if => //.
+    inline{1} RCCA2.O1.extract; wp; sp.
+    if{2}; last by exfalso; smt.
+    if => //.
+      by wp; rnd; skip; progress; smt.
+      sp; if => //.
         by wp; rnd; skip; progress; smt.
         by wp; skip; progress; smt.
-      if{1}.
-        by rnd{1}; skip; progress; smt.
-        by skip; progress; smt.
   qed.
 
-  local equiv RCCA0_RCCA1 :
-    RCCA0.main ~ RCCA1.main : true ==> !RCCA1.abort{2} => ={res}.
+  local equiv RCCA2_RCCA3 :
+    RCCA2.main ~ RCCA3.main : true ==> !RCCA3.abort{2} => ={res}.
   proof.
     fun.
-    swap{1} 11 -3; swap{2} 14 -6.
-    seq 8 8 : 
+    swap{1} 15 -3; swap{2} 14 -6.
+    seq 12 8 : 
      (={b} /\ pms{1} = V.pms{2} /\ c{1} = V.c{2} /\ (pv, h){1} = pp /\
-      (!RCCA1.abort{2} =>
-       ={glob A} /\ t{1} = V.t{2} /\ RO_KEF.m{1} = RCCA1.m{2} /\
+      (!RCCA3.abort{2} =>
+       ={glob A} /\ W.t{1} = V.t{2} /\ RCCA2.m{1} = RCCA3.m{2} /\
        keypair(V.pk, V.sk){2} /\
-       W.sk{1} = V.sk{2} /\ W.keys{1} = V.keys{2} /\ W.labels{1} = V.labels{2} /\
-       (decrypt V.sk (fst pp) V.c = V.pms){2} /\
-       (forall t, in_dom (snd pp, (V.pms, t)) RCCA1.m => mem t V.labels){2})).
+       W.sk{1} = V.sk{2} /\ W.keys{1} = V.keys{2} /\ W.labels{1} = V.labels{2} /\ W.guess{1} = V.guess{2} /\
+       (decrypt (fst pp) V.sk V.c = Some V.pms){2} /\
+       (forall t, in_dom (pp, (V.pms, t)) RCCA3.m => mem t V.labels){2})).
       rnd; simplify.
-      call (_:RCCA1.abort,
+      call (_:RCCA3.abort,
         keypair(V.pk, V.sk){2} /\
-        !V.guess{2} /\ RO_KEF.m{1} = RCCA1.m{2} /\
-        W.sk{1} = V.sk{2} /\ W.keys{1} = V.keys{2} /\ W.labels{1} = V.labels{2} /\
-        (decrypt V.sk (fst pp) V.c = V.pms){2} /\
-        (forall t, in_dom (snd pp, (V.pms, t)) RCCA1.m => 
-           RCCA1.abort \/ mem t V.labels){2}).
+        !V.guess{2} /\ RCCA2.m{1} = RCCA3.m{2} /\
+        W.sk{1} = V.sk{2} /\ W.keys{1} = V.keys{2} /\ W.labels{1} = V.labels{2} /\ W.t{1} = V.t{2} /\ W.guess{1} = V.guess{2} /\
+        (decrypt (fst pp) V.sk V.c = Some V.pms){2} /\
+        (forall t, in_dom (pp, (V.pms, t)) RCCA3.m => 
+           RCCA3.abort \/ mem t V.labels){2}).
       by apply lossless_choose.
-      by apply RCCA0_RCCA1_dec_choose.
-      by progress; apply RCCA0_lossless_dec.
-      by apply RCCA1_dec_preserves_abort.
-      by apply RCCA0_RCCA1_extract_choose.
-      by progress; apply lossless_extract.
+      by apply RCCA2_RCCA3_dec_choose.
+      by progress; apply RCCA2_lossless_dec.
+      by apply RCCA3_dec_preserves_abort.
+      by apply RCCA2_RCCA3_extract_choose.
+      by progress; apply RCCA2_lossless_extract.
       by progress; fun; sp; if; try rnd; skip; smt. 
-      seq 2 2 : 
-       (pk{1} = V.pk{2} /\ W.sk{1} = V.sk{2} /\ keypair(V.pk, V.sk){2} /\
-        RO_KEF.m{1} = Core.empty).
-        inline MS_KEM.init RO_KEF.init MS_KEM.keygen; wp.
-        by call keygen_spec_rel; wp; call (_:true).
+      seq 3 2 : (pk{1} = V.pk{2} /\ W.sk{1} = V.sk{2} /\ keypair(V.pk, V.sk){2}).
+        inline MS_KEM.init MS_KEM.keygen; wp.
+        call keygen_spec_rel; wp; call (_:true).
+        (* RCCA2.sample lossless *)
+        call{1} (_:true ==> true) => //.
+          fun; sp; while true (card labels).
+          intros _; wp; rnd; wp; skip; smt.
+          skip; progress; smt.
         inline V.init; sp; exists * V.sk{2}, V.pk{2}; elim *; intros sk pk.
         by call (enc_spec_rel sk pk (fst pp)); skip; progress; smt.
 
-      inline RO_KEF.extract; wp; sp.
-      case RCCA1.abort{2}.
+      inline RCCA2.O1.extract; wp; sp.
+      case RCCA3.abort{2}.
         (* abort *)
-        call (_:RCCA1.abort, RCCA1.abort{2}).
+        call (_:RCCA3.abort, RCCA3.abort{2}).
           by apply lossless_guess.
           by exfalso; smt.
-          by progress; apply RCCA0_lossless_dec.
-          by apply RCCA1_dec_preserves_abort.
+          by progress; apply RCCA2_lossless_dec.
+          by apply RCCA3_dec_preserves_abort.
           by exfalso; smt.
-          by progress; apply lossless_extract.
+          by progress; apply RCCA2_lossless_extract.
           by progress; fun; sp; if; try rnd; skip; smt.
         wp; rnd; wp; if{1}.
           by rnd; skip; smt.
@@ -775,20 +1468,20 @@ section.
           (* valid *)
           (* REMARK: here is where the validity condition is used *)
           rcondt{1} 1; first by intros _; skip; smt.
-          call (_:RCCA1.abort,
+          call (_:RCCA3.abort,
            keypair(V.pk, V.sk){2} /\
            V.guess{2} /\ 
-           W.sk{1} = V.sk{2} /\ W.keys{1} = V.keys{2} /\ W.labels{1} = V.labels{2} /\
-           eq_except RO_KEF.m{1} RCCA1.m{2} (snd pp, (V.pms, V.t)){2} /\
-           in_dom (snd pp, (V.pms, V.t)){2} RO_KEF.m{1} /\
-           mem (proj RO_KEF.m{1}.[(snd pp, (V.pms, V.t))]){2} V.keys{2} /\
-           decrypt V.sk{2} (fst pp) V.c{2} = V.pms{2}).
+           W.sk{1} = V.sk{2} /\ W.keys{1} = V.keys{2} /\ W.labels{1} = V.labels{2} /\ W.t{1} = V.t{2} /\ W.guess{1} = V.guess{2} /\
+           eq_except RCCA2.m{1} RCCA3.m{2} (pp, (V.pms, V.t)){2} /\
+           in_dom (pp, (V.pms, V.t)){2} RCCA2.m{1} /\
+           mem (proj RCCA2.m{1}.[(pp, (V.pms, V.t))]){2} V.keys{2} /\
+           decrypt (fst pp) V.sk{2} V.c{2} = Some V.pms{2}).
           by apply lossless_guess.
-          by apply RCCA0_RCCA1_dec_guess.
-          by progress; apply RCCA0_lossless_dec.
-          by apply RCCA1_dec_preserves_abort.
-          by apply RCCA0_RCCA1_extract_guess.
-          by progress; apply lossless_extract.
+          by apply RCCA2_RCCA3_dec_guess.
+          by progress; apply RCCA2_lossless_dec.
+          by apply RCCA3_dec_preserves_abort.
+          by apply RCCA2_RCCA3_extract_guess.
+          by progress; apply RCCA2_lossless_extract.
           by intros _; fun; sp; if; try rnd; skip; smt.
           wp; case b{1}.
             by swap{2} 1; rnd; wp; rnd; skip; progress; smt.
@@ -796,57 +1489,91 @@ section.
    
           (* !abort /\ !valid *)  
           call{1} (_:true ==> true).
-            apply (lossless_guess RO_KEF RCCA0.O).
-              by apply RCCA0_lossless_dec.
-              by apply lossless_extract.
+            apply (lossless_guess RCCA2.O1 RCCA2.O2).
+              by apply RCCA2_lossless_dec.
+              by apply RCCA2_lossless_extract.
           call{2} (_:true ==> true).
-            apply (lossless_guess RCCA1.O1 RCCA1.O2).
-              by apply RCCA1_lossless_dec.
-              by fun; sp; if => //; rnd; skip; smt.
-
+            apply (lossless_guess RCCA3.O1 RCCA3.O2).
+              by apply RCCA3_lossless_dec.
+              by apply RCCA3_lossless_extract.
       wp; rnd; wp; if{1}.
         by rnd; skip; progress; smt.
         by rnd{2}; skip; smt.
   qed.
   
-  local lemma Pr_RCCA1_res : forall &m, 
-    Pr[RCCA1.main() @ &m : res] <= 1%r / 2%r.
+  local lemma Pr_RCCA3_res &m : Pr[RCCA3.main() @ &m : res] <= 1%r / 2%r.
   proof.
-    intros &m; bdhoare_deno (_:true) => //. 
+    bdhoare_deno (_:true) => //. 
     fun; rnd; simplify; call (_:true) => //.  
     wp; rnd; rnd; wp; call (_:true) => //.
     inline V.init; call (_:true); wp; call (_:true); wp; call (_:true).
     by skip; progress; try rewrite Bool.Dbool.mu_def; smt.
   qed.
   
-  local lemma Pr_RCCA_RCCA1 : forall &m,
+  local lemma Pr_RCCA_RCCA2 &m :
     Pr[RCCA(KEM(RO_KEF, PMS_KEM), A(RO_KEF)).main() @ &m : res] <=
-    1%r / 2%r + Pr[RCCA1.main() @ &m : RCCA1.abort].
+    Pr[RCCA2.main() @ &m : res] +
+    Pr[RCCA2.main() @ &m : exists pv h t, in_dom ((pv, h), (proj RCCA2.fake.[(pv, t)], t)) RCCA2.m].
   proof.
-   intros &m.
-   apply (Trans _ Pr[RCCA0.main() @ &m : res]).
-   equiv_deno RCCA_RCCA0 => //.
-   apply (Trans _ Pr[RCCA1.main() @ &m : res \/ RCCA1.abort]).
-     by equiv_deno RCCA0_RCCA1; smt.  
-     by rewrite Pr mu_or; smt.
+    apply (Trans _ Pr[RCCA0.main() @ &m : res]).
+    equiv_deno RCCA_RCCA0 => //.
+    rewrite (Pr_RCCA0_RCCA1 &m).
+    apply (Trans _   
+     (Pr[RCCA2.main() @ &m : res] +
+      Pr[RCCA2.main() @ &m : exists pv h t, in_dom ((pv, h), (proj RCCA2.fake.[(pv, t)], t)) RCCA2.m])).
+    apply (Pr_RCCA1_RCCA2 &m).
+    smt.
+  qed.
+
+  local lemma Pr_RCCA2_RCCA3 &m :
+    Pr[RCCA2.main() @ &m : res] <= 1%r / 2%r + Pr[RCCA3.main() @ &m : RCCA3.abort].
+  proof.
+    apply (Trans _ Pr[RCCA3.main() @ &m : res \/ RCCA3.abort]).
+      by equiv_deno RCCA2_RCCA3; smt.  
+      by rewrite Pr mu_or; smt.
+  qed.
+
+  local lemma Pr_RCCA_RCCA3 &m :
+    Pr[RCCA(KEM(RO_KEF, PMS_KEM), A(RO_KEF)).main() @ &m : res] <=
+    1%r / 2%r +
+    Pr[RCCA2.main() @ &m : exists pv h t, in_dom ((pv, h), (proj RCCA2.fake.[(pv, t)], t)) RCCA2.m] +
+    Pr[RCCA3.main() @ &m : RCCA3.abort].
+  proof.
+    apply (Trans _ 
+     (Pr[RCCA2.main() @ &m : res] +
+      Pr[RCCA2.main() @ &m : exists pv h t, in_dom ((pv, h), (proj RCCA2.fake.[(pv, t)], t)) RCCA2.m])).
+    apply (Pr_RCCA_RCCA2 &m).
+    apply (Trans _
+      (1%r / 2%r + Pr[RCCA3.main() @ &m : RCCA3.abort] +
+      Pr[RCCA2.main() @ &m : exists pv h t, in_dom ((pv, h), (proj RCCA2.fake.[(pv, t)], t)) RCCA2.m])).
+    by apply addleM => //; [apply (Pr_RCCA2_RCCA3 &m) | smt].
+    by smt.
   qed.
   
-  
-  (** RCCA1 -> RCCA2 **)
-  
-  local module RCCA2 = {
-    var m : (hash * (pms * label), ms) map
+  (** RCCA3 -> RCCA4 **)
+
+  (*
+   * This game uses two maps m and d to implement the simulation for
+   * the RCCA adversary A. If the simulation fails and the previous
+   * game aborts, then either the pms used to compute the challenge ciphertext
+   * can be obtained from map m using the plaintext-checking oracle, or else
+   * a randomization of the challenge ciphertext can be obtained by a direct
+   * lookup in d.
+   *)  
+  local module RCCA4 = {
+    var m : ((version * hash) * (pms * label), ms) map
     var d : (label, (ms * version * hash * ciphertext)) map
    
     module O1 = {
-      fun extract(p:hash, s:pms * label) : ms = {
+      fun extract(p:version * hash, s:pms * label) : ms = {
         var k : ms;
         var pms : pms;
         var t : label;
         (pms, t) = s;
         if (!in_dom (p, (pms, t)) m) {
           if (in_dom t d /\ 
-              let (ms, pv, h, c) = proj d.[t] in p = h /\ decrypt V.sk pv c = pms) {
+              let (ms, pv, h, c) = proj d.[t] in 
+                p = (pv, h) /\ decrypt pv V.sk c = Some pms) {
             k = let (ms, pv, h, c) = proj d.[t] in ms;
           }
           else k = $key;
@@ -866,13 +1593,15 @@ section.
         if (!mem t V.labels /\ mem p P) { 
           V.labels = add t V.labels;
           (pv, h) = p;
-          if (!(V.guess /\ same_key V.pk (fst pp) pv c /\ h = snd pp /\ t = V.t /\ V.c = c)) {
-            if (in_dom (h, (decrypt V.sk pv c, t)) m) {
-              k = proj m.[(h, (decrypt V.sk pv c, t))];
+          if (!(V.guess /\ p = pp /\ t = V.t /\ V.c = c)) {
+            if (decrypt pv V.sk c <> None /\ 
+                in_dom ((pv, h), (proj (decrypt pv V.sk c), t)) m) {
+              k = proj m.[((pv, h), (proj (decrypt pv V.sk c), t))];
             }
             else k = $key;
             d.[t] = (k, pv, h, c);
-            maybe_k = if (!mem k V.keys) then Some k else None;
+            maybe_k = if (V.guess => !mem k V.keys \/ t <> V.t) 
+                      then Some k else None;
           }
         }
         return maybe_k;
@@ -889,7 +1618,7 @@ section.
       V.init();
       m = Core.empty;
       d = Core.empty;
-      (V.pms, V.c) = PMS_KEM.enc((), V.pk, fst pp);
+      (V.pms, V.c) = PMS_KEM.enc(fst pp, V.pk, ());
       V.t = A.choose(V.pk);
       k0 = $key;
       k1 = $key;
@@ -900,283 +1629,321 @@ section.
     }
   }.
   
-  local equiv RCCA1_RCCA2_extract : 
-    RCCA1.O1.extract ~ RCCA2.O1.extract :
+  local equiv RCCA3_RCCA4_extract : 
+    RCCA3.O1.extract ~ RCCA4.O1.extract :
     ={p, s} /\ 
     ={glob V} /\
     (V.guess{1} => ={V.t}) /\
-    (decrypt V.sk (fst pp) V.c = V.pms){2} /\ 
-    (RCCA1.abort{1} =>
-     (exists t, in_dom (snd pp, (V.pms, t)) RCCA2.m) \/
-     (V.guess /\ in_dom V.t RCCA2.d /\
-      let (k, pv, h, c) = proj RCCA2.d.[V.t] in
-       c <> V.c /\ decrypt V.sk pv c = V.pms)){2} /\
-    (forall t, in_dom t RCCA2.d => mem t V.labels){2} /\
-    (forall h pms t, 
-     (in_dom (h, (pms, t)) RCCA1.m{1} <=>
-     (in_dom (h, (pms, t)) RCCA2.m{2} \/
-      (in_dom t RCCA2.d{2} /\ 
-       let (k, pv, h', c) = proj RCCA2.d{2}.[t] in 
-        h = h' /\ decrypt V.sk{2} pv c = pms)))) /\
-    (forall h pms t, 
-     (in_dom (h, (pms, t)) RCCA1.m{1} => 
-      in_dom (h, (pms, t)) RCCA2.m{2} => 
-      RCCA1.m{1}.[(h, (pms, t))] = RCCA2.m{2}.[(h, (pms, t))])) /\
-    (forall h pms t, 
-     (in_dom (h, (pms, t)) RCCA1.m{1} => 
-      !in_dom (h, (pms, t)) RCCA2.m{2} => 
-        RCCA1.m{1}.[(h, (pms, t))] = 
-        let (k, pv, h', c) = proj RCCA2.d{2}.[t] in Some k))
+    (decrypt (fst pp) V.sk V.c = Some V.pms){2} /\ 
+    (RCCA3.abort{1} =>
+     (exists t, in_dom (pp, (V.pms, t)) RCCA4.m) \/
+     (V.guess /\ in_dom V.t RCCA4.d /\
+      let (k, pv, h, c) = proj RCCA4.d.[V.t] in
+       pv = fst pp /\ h = snd pp /\ c <> V.c /\ decrypt pv V.sk c = Some V.pms)){2} /\
+    (forall t, in_dom t RCCA4.d => mem t V.labels){2} /\
+    (forall p pms t, 
+     (in_dom (p, (pms, t)) RCCA3.m{1} <=>
+     (in_dom (p, (pms, t)) RCCA4.m{2} \/
+      (in_dom t RCCA4.d{2} /\ 
+       let (k, pv, h, c) = proj RCCA4.d{2}.[t] in 
+        pv = fst p /\ h = snd p /\ decrypt pv V.sk{2} c = Some pms)))) /\
+    (forall p pms t, 
+     (in_dom (p, (pms, t)) RCCA3.m{1} => 
+      in_dom (p, (pms, t)) RCCA4.m{2} => 
+      RCCA3.m{1}.[(p, (pms, t))] = RCCA4.m{2}.[(p, (pms, t))])) /\
+    (forall p pms t, 
+     (in_dom (p, (pms, t)) RCCA3.m{1} => 
+      !in_dom (p, (pms, t)) RCCA4.m{2} => 
+        RCCA3.m{1}.[(p, (pms, t))] = 
+        let (k, pv, h, c) = proj RCCA4.d{2}.[t] in Some k))
     ==>
     ={res} /\
     ={glob V} /\
     (V.guess{1} => ={V.t}) /\
-    (decrypt V.sk (fst pp) V.c = V.pms){2} /\ 
-    (RCCA1.abort{1} =>
-     (exists t, in_dom (snd pp, (V.pms, t)) RCCA2.m) \/
-     (V.guess /\ in_dom V.t RCCA2.d /\
-      let (k, pv, h, c) = proj RCCA2.d.[V.t] in
-       c <> V.c /\ decrypt V.sk pv c = V.pms)){2} /\
-    (forall t, in_dom t RCCA2.d => mem t V.labels){2} /\
-    (forall h pms t, 
-     (in_dom (h, (pms, t)) RCCA1.m{1} <=>
-     (in_dom (h, (pms, t)) RCCA2.m{2} \/
-      (in_dom t RCCA2.d{2} /\ 
-       let (k, pv, h', c) = proj RCCA2.d{2}.[t] in 
-        h = h' /\ decrypt V.sk{2} pv c = pms)))) /\
-    (forall h pms t, 
-     (in_dom (h, (pms, t)) RCCA1.m{1} => 
-      in_dom (h, (pms, t)) RCCA2.m{2} => 
-      RCCA1.m{1}.[(h, (pms, t))] = RCCA2.m{2}.[(h, (pms, t))])) /\
-    (forall h pms t, 
-     (in_dom (h, (pms, t)) RCCA1.m{1} => 
-      !in_dom (h, (pms, t)) RCCA2.m{2} => 
-        RCCA1.m{1}.[(h, (pms, t))] = 
-        let (k, pv, h', c) = proj RCCA2.d{2}.[t] in Some k)).
+    (decrypt (fst pp) V.sk V.c = Some V.pms){2} /\ 
+    (RCCA3.abort{1} =>
+     (exists t, in_dom (pp, (V.pms, t)) RCCA4.m) \/
+     (V.guess /\ in_dom V.t RCCA4.d /\
+      let (k, pv, h, c) = proj RCCA4.d.[V.t] in
+       pv = fst pp /\ h = snd pp /\ c <> V.c /\ decrypt pv V.sk c = Some V.pms)){2} /\
+    (forall t, in_dom t RCCA4.d => mem t V.labels){2} /\
+    (forall p pms t, 
+     (in_dom (p, (pms, t)) RCCA3.m{1} <=>
+     (in_dom (p, (pms, t)) RCCA4.m{2} \/
+      (in_dom t RCCA4.d{2} /\ 
+       let (k, pv, h, c) = proj RCCA4.d{2}.[t] in 
+        pv = fst p /\ h = snd p /\ decrypt pv V.sk{2} c = Some pms)))) /\
+    (forall p pms t, 
+     (in_dom (p, (pms, t)) RCCA3.m{1} => 
+      in_dom (p, (pms, t)) RCCA4.m{2} => 
+      RCCA3.m{1}.[(p, (pms, t))] = RCCA4.m{2}.[(p, (pms, t))])) /\
+    (forall p pms t, 
+     (in_dom (p, (pms, t)) RCCA3.m{1} => 
+      !in_dom (p, (pms, t)) RCCA4.m{2} => 
+        RCCA3.m{1}.[(p, (pms, t))] = 
+        let (k, pv, h, c) = proj RCCA4.d{2}.[t] in Some k)).
   proof.
     fun.
     sp; if{1}.
       rcondt{2} 1; first by intros &1; skip; intros &2; progress; smt.
       sp; rcondf{2} 1.
         intros &1; skip; intros &2; progress.
-        by cut W := H1 p{2} pms{2} t{2}; smt.   
+        by cut W := H2 p{2} pms{2} t{2}; smt.   
       wp; rnd; skip; progress.
         by smt.   
-        elim H8; clear H8; intros ?.
+        elim H9; clear H9; intros ?.
           cut W : abortL = true by smt; subst.
-          elim H; last by smt.
+          elim H0; last by smt.
           by intros [t0 ?]; left; exists t0; smt.
           by left; exists t{2}; smt.
-        cut W := H1 h pms0 t0. 
-        case (in_dom (h, (pms0, t0)) RCCA1.m{1}); first by smt.
-        by intros ?; left; smt.
-        elim H8; clear H8; intros ?.
-          by case (in_dom (h, (pms0, t0)) RCCA2.m{2}); smt.
-          cut W := H1 h pms0 t0.
-          cut V : in_dom (h, (pms0, t0)) RCCA1.m{1}.
+        cut W := H2 p0 pms0 t0. 
+        case (in_dom (p0, (pms0, t0)) RCCA3.m{1}) => ?; first by smt.
+        by cut : (p0, (pms0, t0)) = (p, (pms, t)){2}; smt.
+        elim H9; clear H9; intros ?.
+          by case (in_dom (p0, (pms0, t0)) RCCA4.m{2}); smt.
+          cut W := H2 p0 pms0 t0.
+          cut V : in_dom (p0, (pms0, t0)) RCCA3.m{1}.
           by elim W; intros _ X; apply X; smt.
         by smt.
-        by cut W := H2 h pms0 t0; smt.    
-        by cut W := H1 h pms0 t0; cut X := H3 h pms0 t0; smt.
+        by cut W := H3 p0 pms0 t0; smt.    
+        by cut W := H2 p0 pms0 t0; cut X := H4 p0 pms0 t0; smt.
        
      if{2}.
        sp; rcondt{2} 1; first by intros &1; skip; intros &2; progress; smt.
        wp; skip; progress.
          by smt.
-         elim H6; clear H6; intros ?.
+         elim H7; clear H7; intros ?.
            cut W : abortL = true by smt; subst.
-           elim H; last by smt.
+           elim H0; last by smt.
            by intros [t0 ?]; left; exists t0; smt.
            by left; exists t{2}; smt.
-         by cut W := H1 h pms0 t0; smt. 
-         elim H6; clear H6; intros ?.
-         case (in_dom (h, (pms0, t0)) RCCA2.m{2}); first by smt.
-         by intros ?; cut V : (h, (pms0, t0)) = (p, (pms, t)){2}; smt.
-         cut W := H1 h pms0 t0.
+         by cut W := H2 p0 pms0 t0; smt. 
+         elim H7; clear H7; intros ?.
+         case (in_dom (p0, (pms0, t0)) RCCA4.m{2}); first by smt.
+         by intros ?; cut V : (p0, (pms0, t0)) = (p, (pms, t)){2}; smt.
+         cut W := H2 p0 pms0 t0.
          by elim W; intros _ X; apply X; smt.
          by smt.
          by smt.
-      by wp; skip; smt.
+      by wp; skip; progress; smt.
   qed.
   
-  local equiv RCCA1_RCCA2_dec :
-    RCCA1.O2.dec ~ RCCA2.O2.dec : 
+  local equiv RCCA3_RCCA4_dec :
+    RCCA3.O2.dec ~ RCCA4.O2.dec : 
     ={p, t, c} /\ 
     ={glob V} /\
     (V.guess{1} => ={V.t}) /\
-    (decrypt V.sk (fst pp) V.c = V.pms){2} /\ 
-    (RCCA1.abort{1} =>
-     (exists t, in_dom (snd pp, (V.pms, t)) RCCA2.m) \/
-     (V.guess /\ in_dom V.t RCCA2.d /\
-      let (k, pv, h, c) = proj RCCA2.d.[V.t] in
-       c <> V.c /\ decrypt V.sk pv c = V.pms)){2} /\
-    (forall t, in_dom t RCCA2.d => mem t V.labels){2} /\
-    (forall h pms t, 
-     (in_dom (h, (pms, t)) RCCA1.m{1} <=>
-     (in_dom (h, (pms, t)) RCCA2.m{2} \/
-      (in_dom t RCCA2.d{2} /\ 
-       let (k, pv, h', c) = proj RCCA2.d{2}.[t] in 
-        h = h' /\ decrypt V.sk{2} pv c = pms)))) /\
-    (forall h pms t, 
-     (in_dom (h, (pms, t)) RCCA1.m{1} => 
-      in_dom (h, (pms, t)) RCCA2.m{2} => 
-      RCCA1.m{1}.[(h, (pms, t))] = RCCA2.m{2}.[(h, (pms, t))])) /\
-    (forall h pms t, 
-     (in_dom (h, (pms, t)) RCCA1.m{1} => 
-      !in_dom (h, (pms, t)) RCCA2.m{2} => 
-        RCCA1.m{1}.[(h, (pms, t))] = 
-        let (k, pv, h', c) = proj RCCA2.d{2}.[t] in Some k))
+    (decrypt (fst pp) V.sk V.c = Some V.pms){2} /\ 
+    (RCCA3.abort{1} =>
+     (exists t, in_dom (pp, (V.pms, t)) RCCA4.m) \/
+     (V.guess /\ in_dom V.t RCCA4.d /\
+      let (k, pv, h, c) = proj RCCA4.d.[V.t] in
+       pv = fst pp /\ h = snd pp /\ c <> V.c /\ decrypt pv V.sk c = Some V.pms)){2} /\
+    (forall t, in_dom t RCCA4.d => mem t V.labels){2} /\
+    (forall p pms t, 
+     (in_dom (p, (pms, t)) RCCA3.m{1} <=>
+     (in_dom (p, (pms, t)) RCCA4.m{2} \/
+      (in_dom t RCCA4.d{2} /\ 
+       let (k, pv, h, c) = proj RCCA4.d{2}.[t] in 
+        pv = fst p /\ h = snd p /\ decrypt pv V.sk{2} c = Some pms)))) /\
+    (forall p pms t, 
+     (in_dom (p, (pms, t)) RCCA3.m{1} => 
+      in_dom (p, (pms, t)) RCCA4.m{2} => 
+      RCCA3.m{1}.[(p, (pms, t))] = RCCA4.m{2}.[(p, (pms, t))])) /\
+    (forall p pms t, 
+     (in_dom (p, (pms, t)) RCCA3.m{1} => 
+      !in_dom (p, (pms, t)) RCCA4.m{2} => 
+        RCCA3.m{1}.[(p, (pms, t))] = 
+        let (k, pv, h, c) = proj RCCA4.d{2}.[t] in Some k))
     ==>
     ={res} /\
     ={glob V} /\
     (V.guess{1} => ={V.t}) /\
-    (decrypt V.sk (fst pp) V.c = V.pms){2} /\ 
-    (RCCA1.abort{1} =>
-     (exists t, in_dom (snd pp, (V.pms, t)) RCCA2.m) \/
-     (V.guess /\ in_dom V.t RCCA2.d /\
-      let (k, pv, h, c) = proj RCCA2.d.[V.t] in
-       c <> V.c /\ decrypt V.sk pv c = V.pms)){2} /\
-    (forall t, in_dom t RCCA2.d => mem t V.labels){2} /\
-    (forall h pms t, 
-     (in_dom (h, (pms, t)) RCCA1.m{1} <=>
-     (in_dom (h, (pms, t)) RCCA2.m{2} \/
-      (in_dom t RCCA2.d{2} /\ 
-       let (k, pv, h', c) = proj RCCA2.d{2}.[t] in 
-        h = h' /\ decrypt V.sk{2} pv c = pms)))) /\
-    (forall h pms t, 
-     (in_dom (h, (pms, t)) RCCA1.m{1} => 
-      in_dom (h, (pms, t)) RCCA2.m{2} => 
-      RCCA1.m{1}.[(h, (pms, t))] = RCCA2.m{2}.[(h, (pms, t))])) /\
-    (forall h pms t, 
-     (in_dom (h, (pms, t)) RCCA1.m{1} => 
-      !in_dom (h, (pms, t)) RCCA2.m{2} => 
-        RCCA1.m{1}.[(h, (pms, t))] = 
-        let (k, pv, h', c) = proj RCCA2.d{2}.[t] in Some k)).
+    (decrypt (fst pp) V.sk V.c = Some V.pms){2} /\ 
+    (RCCA3.abort{1} =>
+     (exists t, in_dom (pp, (V.pms, t)) RCCA4.m) \/
+     (V.guess /\ in_dom V.t RCCA4.d /\
+      let (k, pv, h, c) = proj RCCA4.d.[V.t] in
+       pv = fst pp /\ h = snd pp /\ c <> V.c /\ decrypt pv V.sk c = Some V.pms)){2} /\
+    (forall t, in_dom t RCCA4.d => mem t V.labels){2} /\
+    (forall p pms t, 
+     (in_dom (p, (pms, t)) RCCA3.m{1} <=>
+     (in_dom (p, (pms, t)) RCCA4.m{2} \/
+      (in_dom t RCCA4.d{2} /\ 
+       let (k, pv, h, c) = proj RCCA4.d{2}.[t] in 
+        pv = fst p /\ h = snd p /\ decrypt pv V.sk{2} c = Some pms)))) /\
+    (forall p pms t, 
+     (in_dom (p, (pms, t)) RCCA3.m{1} => 
+      in_dom (p, (pms, t)) RCCA4.m{2} => 
+      RCCA3.m{1}.[(p, (pms, t))] = RCCA4.m{2}.[(p, (pms, t))])) /\
+    (forall p pms t, 
+     (in_dom (p, (pms, t)) RCCA3.m{1} => 
+      !in_dom (p, (pms, t)) RCCA4.m{2} => 
+        RCCA3.m{1}.[(p, (pms, t))] = 
+        let (k, pv, h, c) = proj RCCA4.d{2}.[t] in Some k)).
   proof.
     fun.
     wp; sp; if => //.
-    inline{1} RCCA1.O1.extract.
+    inline{1} RCCA3.O1.extract.
     sp; if => //; first by smt.
       if{1}.
         if{2}.
           by exfalso; smt.
           wp; rnd; skip; progress.
             by smt.
-            elim H12; clear H12; intros ?.
-            cut X : abortL = true by smt; subst.
-            elim H; last by smt.
-            by intros [t0 ?]; left; exists t0; smt.
-            by right; smt.
             by smt.
-            case (in_dom (h0, (pms0, t0)) RCCA1.m{1}); first by smt.
-            by intros ?; cut Z : 
-              (h0, (pms0, t0)) =
-              (h{2}, (decrypt V.sk{2} pv{2} c{2}, t{2})); smt.
-            elim H12; clear H12; intros ?; first by smt.
-            case (t0 = t{2}).
-              intros ?; subst; elim H12; clear H12; intros X Y.
+            by smt.
+            elim H13; clear H13; intros ?.
+            by smt.
+            case (t0 = t{2}) => ?.
+              subst; elim H13; clear H13; intros X Y.
               by generalize Y; rewrite /_.[_] Core.get_setE; smt.
-              intros ?.
-              cut L : (in_dom (h0, (pms0, t0)) RCCA1.m{1}); last by smt.
-              rewrite H1.
-              cut L : (in_dom t0 RCCA2.d{2} /\
-                let (k0, pv0, h', c0) = proj RCCA2.d{2}.[t0] in
-                  h0 = h' /\ decrypt V.sk{2} pv0 c0 = pms0).
+              cut L : (in_dom (p0, (pms0, t0)) RCCA3.m{1}); last by smt.
+              rewrite H2.
+              cut L : (in_dom t0 RCCA4.d{2} /\
+                let (k0, pv0, h0, c0) = proj RCCA4.d{2}.[t0] in
+                  h0 = snd p0 /\ decrypt pv0 V.sk{2} c0 = Some pms0).
               split; first by smt.
-              by generalize H12; rewrite /_.[_] Core.get_setN; smt.
+              by generalize H13; rewrite /_.[_] Core.get_setN; smt.
+            by right; smt.   
             by smt.
+
+          if{2}.
+          sp; if{1}; first by exfalso; smt.
+          wp; skip; progress.
             by smt.
-            by case ((h, (decrypt V.sk pv c, t)){2} = (h0, (pms0, t0))); smt.
+            elim H12; clear H12; intros ?; first by smt.
+            right; split; first by smt.
+            split; first by smt.
+            cut -> : t{2} = V.t{2} by smt.
+            rewrite /_.[_] Core.get_setE; smt.
+
+            by smt.
+
+            case (in_dom (p0, (pms0, t0)) RCCA4.m{2}) => //= ?.
+            case (t0 = t{2}) => ?.
+              subst; split; smt.
+              split; first by smt.
+              rewrite /_.[_] /_.[_] Core.get_setN; smt.
+
+            elim H12 => ?; clear H12; first by smt.
+              cut L : (in_dom (p0, (pms0, t0)) RCCA3.m{1}); last by smt.
+              rewrite H2.
+              case (t0 = t{2}) => ?.
+                subst; elim H13; clear H13 => X Y.
+                by generalize Y; rewrite /_.[_] Core.get_setE; smt.
+
+                right.
+                elim H13; clear H13 => X Y.
+                by generalize X Y; rewrite /_.[_] /_.[_] !Core.get_setN; smt.
+
+            by smt.
     
-      (* similarly *)
-      rcondt{2} 1; first by intros &1; skip; intros &2; progress; smt.
-      wp; skip; progress.
-        by smt.
-        elim H8; clear H8; intros ?.
-        cut X : abortL = true by smt; subst.
-        elim H; last by smt.
-        by intros [t0 ?]; left; exists t0; smt.
-        by right; smt.
-        by smt.
-        by smt.
-        elim H8; clear H8; first by smt.
-        case (t0 = t{2}); first by smt.
-          intros ? [? ?].
-          case ((h, (decrypt V.sk pv c, t)){2} = (h0, (pms0, t0))).
-            by smt.
-            intros ?; rewrite H1; right; split; first by smt.
-            by generalize H10; rewrite /_.[_] Core.get_setN; smt.
-        by smt.
+         sp; if{1}; last by exfalso; smt.
+         wp; rnd; skip; progress.
+           by smt.
+           elim H14 => ?; clear H14; first by smt.
+           right; split; first by smt.
+           split; first by smt.
+           cut -> : t{2} = V.t{2} by smt.
+           rewrite /_.[_] Core.get_setE; smt.
+
+           by smt.
+
+           case (in_dom (p0, (pms0, t0)) RCCA4.m{2}) => //= ?.
+           case ((p0, (pms0, t0)) = ((pv, h){2}, (proj (decrypt pv{2} V.sk{2} c{2}), t{2}))) => ?.
+              split; first by smt.
+              cut -> : (t0 = t){2} by smt.
+              rewrite /_.[_] Core.get_setE; smt.
+              cut L : (in_dom (p0, (pms0, t0)) RCCA3.m{1}) by smt.
+              split; first by smt.
+              by generalize H14; rewrite /_.[_] Core.get_setN; smt.
+
+            elim H14 => ?; clear H14; first by smt.
+
+            elim H15; clear H15 => X Y.
+            case ((p0, (pms0, t0)) = ((pv, h){2}, (proj (decrypt pv{2} V.sk{2} c{2}), t{2}))) => ?.
+              by smt.
+
+              cut L : (in_dom (p0, (pms0, t0)) RCCA3.m{1}); last by smt.
+              rewrite H2.
+              case (in_dom (p0, (pms0, t0)) RCCA4.m{2}) => //= ?.
+              case (t0 = t{2}) => ?.
+                subst; generalize Y; rewrite /_.[_] Core.get_setE proj_some; smt.                   generalize Y; rewrite /_.[_] Core.get_setN; smt.
+
+             by smt.
+             cut : decrypt pv{2} V.sk{2} c{2} <> None by smt.
+             case (t0 = t{2}) => ?; smt.
 
       by skip; progress; smt.
   qed.
   
-  local equiv RCCA1_RCCA2 :
-    RCCA1.main ~ RCCA2.main : 
+  local equiv RCCA3_RCCA4 :
+    RCCA3.main ~ RCCA4.main : 
     true ==>
-    RCCA1.abort{1} =>
-      (exists t, in_dom (snd pp, (V.pms, t)) RCCA2.m){2} \/
-      (in_dom V.t RCCA2.d /\
-       let (k, pv, h, c) = proj RCCA2.d.[V.t] in
-         c <> V.c /\ decrypt V.sk pv c = V.pms){2}.
+    RCCA3.abort{1} =>
+      (exists t, in_dom (pp, (V.pms, t)) RCCA4.m){2} \/
+      (in_dom V.t RCCA4.d /\
+       let (k, pv, h, c) = proj RCCA4.d.[V.t] in
+         pv = fst pp /\ h = snd pp /\ c <> V.c /\ decrypt pv V.sk c = Some V.pms){2}.
   proof.
     fun.
     rnd{1}.
     call (_:
      ={glob V} /\
      (V.guess{1} => ={V.t}) /\
-     (decrypt V.sk (fst pp) V.c = V.pms){2} /\ 
-     (RCCA1.abort{1} =>
-      (exists t, in_dom (snd pp, (V.pms, t)) RCCA2.m) \/
-      (V.guess /\ in_dom V.t RCCA2.d /\
-       let (k, pv, h, c) = proj RCCA2.d.[V.t] in
-        c <> V.c /\ decrypt V.sk pv c = V.pms)){2} /\
-     (forall t, in_dom t RCCA2.d => mem t V.labels){2} /\
-     (forall h pms t, 
-      (in_dom (h, (pms, t)) RCCA1.m{1} <=>
-      (in_dom (h, (pms, t)) RCCA2.m{2} \/
-       (in_dom t RCCA2.d{2} /\ 
-        let (k, pv, h', c) = proj RCCA2.d{2}.[t] in 
-         h = h' /\ decrypt V.sk{2} pv c = pms)))) /\
-     (forall h pms t, 
-      (in_dom (h, (pms, t)) RCCA1.m{1} => 
-       in_dom (h, (pms, t)) RCCA2.m{2} => 
-       RCCA1.m{1}.[(h, (pms, t))] = RCCA2.m{2}.[(h, (pms, t))])) /\
-     (forall h pms t, 
-      (in_dom (h, (pms, t)) RCCA1.m{1} => 
-       !in_dom (h, (pms, t)) RCCA2.m{2} => 
-         RCCA1.m{1}.[(h, (pms, t))] = 
-         let (k, pv, h', c) = proj RCCA2.d{2}.[t] in Some k))).
-      by apply RCCA1_RCCA2_dec.
-      by apply RCCA1_RCCA2_extract.
+     (decrypt (fst pp) V.sk  V.c = Some V.pms){2} /\
+     (RCCA3.abort{1} =>
+      (exists t, in_dom (pp, (V.pms, t)) RCCA4.m) \/
+      (V.guess /\ in_dom V.t RCCA4.d /\
+       let (k, pv, h, c) = proj RCCA4.d.[V.t] in
+        pv = fst pp /\ h = snd pp /\ c <> V.c /\ decrypt pv V.sk c = Some V.pms)){2} /\
+     (forall t, in_dom t RCCA4.d => mem t V.labels){2} /\
+     (forall p pms t, 
+      (in_dom (p, (pms, t)) RCCA3.m{1} <=>
+      (in_dom (p, (pms, t)) RCCA4.m{2} \/
+       (in_dom t RCCA4.d{2} /\ 
+        let (k, pv, h, c) = proj RCCA4.d{2}.[t] in 
+         pv = fst p /\ h = snd p /\ decrypt pv V.sk{2} c = Some pms)))) /\
+     (forall p pms t, 
+      (in_dom (p, (pms, t)) RCCA3.m{1} => 
+       in_dom (p, (pms, t)) RCCA4.m{2} => 
+       RCCA3.m{1}.[(p, (pms, t))] = RCCA4.m{2}.[(p, (pms, t))])) /\
+     (forall p pms t, 
+      (in_dom (p, (pms, t)) RCCA3.m{1} => 
+       !in_dom (p, (pms, t)) RCCA4.m{2} => 
+         RCCA3.m{1}.[(p, (pms, t))] = 
+         let (k, pv, h, c) = proj RCCA4.d{2}.[t] in Some k))).
+      by apply RCCA3_RCCA4_dec.
+      by apply RCCA3_RCCA4_extract.
     wp; rnd; rnd; wp.
     call (_:
      ={glob V} /\
      (V.guess{1} => ={V.t}) /\
-     (decrypt V.sk (fst pp) V.c = V.pms){2} /\ 
-     (RCCA1.abort{1} =>
-      (exists t, in_dom (snd pp, (V.pms, t)) RCCA2.m) \/
-      (V.guess /\ in_dom V.t RCCA2.d /\
-       let (k, pv, h, c) = proj RCCA2.d.[V.t] in
-        c <> V.c /\ decrypt V.sk pv c = V.pms)){2} /\
-     (forall t, in_dom t RCCA2.d => mem t V.labels){2} /\
-     (forall h pms t, 
-      (in_dom (h, (pms, t)) RCCA1.m{1} <=>
-      (in_dom (h, (pms, t)) RCCA2.m{2} \/
-       (in_dom t RCCA2.d{2} /\ 
-        let (k, pv, h', c) = proj RCCA2.d{2}.[t] in 
-         h = h' /\ decrypt V.sk{2} pv c = pms)))) /\
-     (forall h pms t, 
-      (in_dom (h, (pms, t)) RCCA1.m{1} => 
-       in_dom (h, (pms, t)) RCCA2.m{2} => 
-       RCCA1.m{1}.[(h, (pms, t))] = RCCA2.m{2}.[(h, (pms, t))])) /\
-     (forall h pms t, 
-      (in_dom (h, (pms, t)) RCCA1.m{1} => 
-       !in_dom (h, (pms, t)) RCCA2.m{2} => 
-         RCCA1.m{1}.[(h, (pms, t))] = 
-         let (k, pv, h', c) = proj RCCA2.d{2}.[t] in Some k))).
-      by apply RCCA1_RCCA2_dec.
-      by apply RCCA1_RCCA2_extract. 
+     (decrypt (fst pp) V.sk V.c = Some V.pms){2} /\ 
+     (RCCA3.abort{1} =>
+      (exists t, in_dom (pp, (V.pms, t)) RCCA4.m) \/
+      (V.guess /\ in_dom V.t RCCA4.d /\
+       let (k, pv, h, c) = proj RCCA4.d.[V.t] in
+        pv = fst pp /\ h = snd pp /\ c <> V.c /\ decrypt pv V.sk c = Some V.pms)){2} /\
+     (forall t, in_dom t RCCA4.d => mem t V.labels){2} /\
+     (forall p pms t, 
+      (in_dom (p, (pms, t)) RCCA3.m{1} <=>
+      (in_dom (p, (pms, t)) RCCA4.m{2} \/
+       (in_dom t RCCA4.d{2} /\ 
+        let (k, pv, h, c) = proj RCCA4.d{2}.[t] in 
+         pv = fst p /\ h = snd p /\ decrypt pv V.sk{2} c = Some pms)))) /\
+     (forall p pms t, 
+      (in_dom (p, (pms, t)) RCCA3.m{1} => 
+       in_dom (p, (pms, t)) RCCA4.m{2} => 
+       RCCA3.m{1}.[(p, (pms, t))] = RCCA4.m{2}.[(p, (pms, t))])) /\
+     (forall p pms t, 
+      (in_dom (p, (pms, t)) RCCA3.m{1} => 
+       !in_dom (p, (pms, t)) RCCA4.m{2} => 
+         RCCA3.m{1}.[(p, (pms, t))] = 
+         let (k, pv, h, c) = proj RCCA4.d{2}.[t] in Some k))).
+      by apply RCCA3_RCCA4_dec.
+      by apply RCCA3_RCCA4_extract. 
     seq 2 2 : (={V.pk, V.sk} /\ keypair(V.pk, V.sk){1}).
       by call keygen_spec_rel; call (_:true); skip.
       exists * V.pk{1}, V.sk{1}; elim *; intros pk sk.
@@ -1184,72 +1951,78 @@ section.
       inline V.init; wp; skip; progress; smt.
   qed.
   
-  local lemma Pr_RCCA1_RCCA2 : forall &m,
-    Pr[RCCA1.main() @ &m : RCCA1.abort] <=
-    Pr[RCCA2.main() @ &m : exists t, in_dom (snd pp, (V.pms, t)) RCCA2.m] +  
-    Pr[RCCA2.main() @ &m : let (k, pv, h, c) = proj RCCA2.d.[V.t] in
-       c <> V.c /\ decrypt V.sk pv c = V.pms].
+  local lemma Pr_RCCA3_RCCA4 &m :
+    Pr[RCCA3.main() @ &m : RCCA3.abort] <=
+    Pr[RCCA4.main() @ &m : exists t, in_dom (pp, (V.pms, t)) RCCA4.m] +  
+    Pr[RCCA4.main() @ &m : let (k, pv, h, c) = proj RCCA4.d.[V.t] in
+       pv = fst pp /\ h = snd pp /\ c <> V.c /\ decrypt pv V.sk c = Some V.pms].
   proof.
-    intros &m.
     apply (Trans _ 
-      Pr[RCCA2.main() @ &m : 
-       (exists t, in_dom (snd pp, (V.pms, t)) RCCA2.m) \/
-       let (k, pv, h, c) = proj RCCA2.d.[V.t] in
-         c <> V.c /\ decrypt V.sk pv c = V.pms]).
-      by equiv_deno RCCA1_RCCA2; smt.  
+      Pr[RCCA4.main() @ &m : 
+       (exists t, in_dom (pp, (V.pms, t)) RCCA4.m) \/
+       let (k, pv, h, c) = proj RCCA4.d.[V.t] in
+         pv = fst pp /\ h = snd pp /\ c <> V.c /\ decrypt pv V.sk c = Some V.pms]).
+      by equiv_deno RCCA3_RCCA4; smt.  
       rewrite Pr mu_or.
       cut X : forall (x y z), 0%r <= z => x <= y => x - z <= y by smt.
     by apply X; [smt | apply Refl].
   qed.
   
   
-  (** RCCA2 -> OW_PCA **)
+  (** RCCA4 -> OW_PCA **)
+  import Inner_KEM.
+
+  (* 
+   * This module implements auxiliary procedures used in the reduction
+   * to OW_PCA and NR_PCA, and the extract and decryption oracles (the
+   * same are used in both reductions).
+   *)
   local module Find(PCO:PCA.Oracle) = {
-    var m : (hash * (pms * label), ms) map
+    var m : ((version * hash) * (pms * label), ms) map
     var d : (label, (ms * version * hash * ciphertext)) map
     var pk : pkey
   
     (* Private procedures *)
     fun find(pv:version, c:ciphertext, h:hash, t:label) : pms option = {
-      var h' : hash;
+      var p' : version * hash;
       var s : pms * label;
       var pms : pms;
       var t' : label;
       var found : bool;
-      var q : (hash * (pms * label)) set;
+      var q : ((version * hash) * (pms * label)) set;
       var maybe_pms : pms option = None;
       q = dom(m);
       while (q <> FSet.empty /\ maybe_pms = None) {
-        (h',  s) = pick q;
-        q = rm (h', s) q;
+        (p',  s) = pick q;
+        q = rm (p', s) q;
         (pms, t') = s;
-        found = PCO.check((), pms, pv, c);
-        maybe_pms = if found /\ h = h' /\ t = t' then Some pms else None; 
+        found = PCO.check(pv, pms, (), c);
+        if (found /\ pv = fst p' /\ h = snd p' /\ t = t') maybe_pms = Some pms; 
       }
       return maybe_pms;
     }
   
     fun find_any(pv:version, c:ciphertext) : pms option = {
-      var h' : hash;
+      var p' : version * hash;
       var s : pms * label;
       var pms : pms;
       var t' : label;
       var found : bool;
-      var q : (hash * (pms * label)) set;
+      var q : ((version * hash) * (pms * label)) set;
       var maybe_pms : pms option = None;
       q = dom(m);
       while (q <> FSet.empty /\ maybe_pms = None) {
-        (h',  s) = pick q;
-        q = rm (h', s) q;
+        (p',  s) = pick q;
+        q = rm (p', s) q;
         (pms, t') = s;
-        found = PCO.check((), pms, pv, c);
-        maybe_pms = if found then Some pms else None; 
+        found = PCO.check(pv, pms, (), c);
+        if (found) maybe_pms = Some pms;
       }
       return maybe_pms;
     }
 
     module O1 = {
-      fun extract(p:hash, s:pms * label) : ms = {
+      fun extract(p:version * hash, s:pms * label) : ms = {
         var k : ms;
         var pms : pms;
         var t : label;
@@ -1260,8 +2033,8 @@ section.
         (pms, t) = s;
         if (!in_dom (p, (pms, t)) m) {
           (k, pv, h, c) = proj d.[t];
-          found = PCO.check((), pms, pv, c);
-          if (in_dom t d /\ p = h /\ found) {
+          found = PCO.check(pv, pms, (), c);
+          if (in_dom t d /\ p = (pv, h) /\ found) {
             k = let (ms, pv, h, c) = proj d.[t] in ms;
           }
           else k = $key;
@@ -1282,38 +2055,36 @@ section.
         if (!mem t V.labels /\ mem p P) { 
           V.labels = add t V.labels;
           (pv, h) = p;
-          if (!(V.guess /\ same_key pk (fst pp) pv c /\ h = snd pp /\ t = V.t /\ V.c = c)) {
+          if (!(V.guess /\ p = pp /\ t = V.t /\ V.c = c)) {
             maybe_pms = find(pv, c, h, t);
-            if (maybe_pms <> None) k = proj m.[(h, (proj maybe_pms, t))];
+            if (maybe_pms <> None) k = proj m.[((pv, h), (proj maybe_pms, t))];
             else k = $key;
             d.[t] = (k, pv, h, c);
-            maybe_k = if (!mem k V.keys) then Some k else None;
+            maybe_k = if (V.guess => !mem k V.keys \/ t <> V.t) 
+                      then Some k else None;
           }
         }
         return maybe_k;
       }
     }
   }.
- 
+
+  (* Adversary used in the reduction to OW_PCA *)
   local module B(PCO:PCA.Oracle) = {  
     module F = Find(PCO)
     module A = A(Find(PCO).O1, Find(PCO).O2)
    
-    fun choose(pk:pkey) : version = {
-      var t : label;
-      V.init();
-      Find.m = Core.empty;
-      Find.d = Core.empty;
-      Find.pk = pk;
-      V.t = A.choose(pk);
-      return (fst pp);
-    }
+    fun choose(pk:pkey) : unit = { Find.pk = pk; }
   
     fun guess(c:ciphertext) : pms = {
       var maybe_pms : pms option;
       var k0, k1 : ms;
       var b' : bool;
+      V.init();
       V.c = c;
+      Find.m = Core.empty;
+      Find.d = Core.empty;
+      V.t = A.choose(Find.pk);
       k0 = $key;
       k1 = $key;
       V.keys = add k0 (add k1 V.keys);
@@ -1325,10 +2096,10 @@ section.
   }.
 
   local module O = {
-    fun check(p:unit, k:pms, t:version, c:ciphertext) : bool = {
-      var k' : pms;
-      k' = decrypt PCA.V.sk t c;
-      return (k' = k);
+    fun check(p:version, k:pms, t:unit, c:ciphertext) : bool = {
+      var maybe_k : pms option;
+      maybe_k = decrypt p PCA.V.sk c;
+      return (maybe_k = Some k);
     }
   }.
  
@@ -1342,8 +2113,8 @@ section.
       var c : ciphertext;
       PMS_KEM.init();
       (pk, PCA.V.sk) = PMS_KEM.keygen();
-      (k, c) = PMS_KEM.enc((), pk, fst pp);
-      t = B.choose(pk);
+      (k, c) = PMS_KEM.enc(fst pp, pk, ());
+      B.choose(pk);
       k' = B.guess(c);
       return (k = k');
     }
@@ -1355,7 +2126,7 @@ section.
     ={res} /\ ={glob PCA.V}.
   proof.
     fun.
-    wp; exists * PCA.V.sk{2}, t{2}, c{2}; elim *; intros sk pv c.
+    wp; exists * p{2}, PCA.V.sk{2}, c{2}; elim *; intros pv sk c.
     by call{2} (dec_spec sk pv c).
   qed.
 
@@ -1365,96 +2136,115 @@ section.
     fun.
     swap{1} 3 1.
     inline PCA.OW_PCA(PMS_KEM, B).A.guess OW_PCA0.B.guess.
-    eqobs_in (={glob PCA.V}) true : (={k,k',glob Find, glob PCA.V}).
-    apply OW_PCA0_OW_PCA_check.
-    seq 3 3 : 
-     (={pk, glob PCA.V, glob A, glob Find, t} /\ 
-      t{1} = fst pp /\ keypair(pk, PCA.V.sk){2}).
-    inline PCA.OW_PCA(PMS_KEM, B).A.choose OW_PCA0.B.choose; wp.
-    call (_: ={glob PCA.V, glob Find}) => //.
-      fun.
-      eqobs_in true (={glob PCA.V}) : (={maybe_k, glob Find, glob PCA.V}).
-      apply OW_PCA0_OW_PCA_check.
-      fun.
-      eqobs_in (={glob PCA.V}) true : (={k, glob Find, glob PCA.V}).
-      apply OW_PCA0_OW_PCA_check.
-    by inline V.init; wp; call keygen_spec_rel; call (_:true).
-    exists * PCA.V.sk{1}, pk{1}, t{1}; elim *; intros sk pk t.
-    by call (enc_spec_rel sk pk t).
-  qed.
-
-  local lemma check_spec : forall _k _t _c,
+    eqobs_in (={glob PCA.V}) true : (={k,k',glob Find,glob PCA.V});
+      first by apply OW_PCA0_OW_PCA_check.
+    seq 3 3 : (={pk, glob PCA.V, Find.pk} /\ keypair(pk, PCA.V.sk){2}).
+    inline PCA.OW_PCA(PMS_KEM, B).A.choose OW_PCA0.B.choose.
+    wp; call keygen_spec_rel; call (_:true) => //.
+    exists * PCA.V.sk{1}, pk{1}; elim *; intros sk pk.
+    call (enc_spec_rel sk pk (fst pp)).
+    wp; skip; progress.
+    cut X : forall x, tt = x by smt; apply X.
+ qed.
+ 
+  local lemma check_spec _p _k _c :
     bd_hoare 
     [ O.check : 
-      k = _k /\ t = _t /\ c = _c ==>
-      res <=> _k = decrypt PCA.V.sk _t _c ] = 1%r.
+      p = _p /\ k = _k /\ c = _c ==>
+      res <=> decrypt _p PCA.V.sk _c = Some _k ] = 1%r.
   proof.
-    by progress; fun; wp.
+    by fun; wp; skip; smt.
   qed.
-  
-  local lemma find_any_spec : forall _pv _c,
+
+  local lemma find_any_spec _pv _c :
     bd_hoare 
     [ Find(O).find_any : 
       pv = _pv /\ c = _c ==> 
-      let pms = decrypt PCA.V.sk _pv _c in
-       ((exists h t, in_dom (h, (pms, t)) Find.m) <=> res = Some pms) /\
-       (res <> None => res = Some pms)] = 1%r.
+      let maybe = decrypt _pv PCA.V.sk _c in
+       res = 
+       if (exists h t, in_dom (h, (proj maybe, t)) Find.m) then maybe
+       else None ] = 1%r.
   proof.
-    progress; fun; sp.
+    fun; sp.
     while  
-     (let pms = decrypt PCA.V.sk pv c in
-      (forall x, mem x q => in_dom x Find.m) /\
-      (forall x, 
-       in_dom x Find.m => !mem x q => maybe_pms = None => pms <> fst (snd x)) /\
-      (maybe_pms <> None =>
-       (exists h t, in_dom (h, (pms, t)) Find.m) /\ maybe_pms = Some pms))
+     ((forall x, mem x q => in_dom x Find.m) /\
+      let maybe = decrypt pv PCA.V.sk c in
+        (maybe_pms <> None => 
+         maybe_pms = maybe /\ maybe <> None /\ 
+         exists h t, in_dom (h, (proj maybe, t)) Find.m) /\
+        forall x, 
+          in_dom x Find.m => !mem x q => maybe_pms = None => 
+           maybe <> Some (fst (snd x)))
      (card q).
        intros z; sp; wp. 
        exists * pms, pv, c; elim *; intros pms pv c.
-       by call (check_spec pms pv c); skip; progress; smt. 
-     by wp; skip; progress; smt.
+       call (check_spec pv pms c); skip; progress; smt. 
+
+    wp; skip; intros &1; progress => //.
+      by smt.
+      by smt.
+      case (decrypt pv PCA.V.sk c = None){1} => ?.
+        by smt.
+        case (maybe_pms0 = None) => ?; last by smt.
+        cut : forall h pms t,
+          in_dom (h, (pms, t)) Find.m{1} =>
+          decrypt pv{1} PCA.V.sk{1} c{1} <> Some pms by smt => ?.
+        cut : !exists h t,
+          in_dom (h, (proj (decrypt pv{1} PCA.V.sk{1} c{1}), t)) Find.m{1} /\
+          decrypt pv{1} PCA.V.sk{1} c{1} <> None by smt.
+        by smt.
   qed.
   
-  local lemma find_spec : forall _pv _c _h _t,
+  local lemma find_spec _pv _c _h _t :
     bd_hoare 
     [ Find(O).find : 
       pv = _pv /\ c = _c /\ h = _h /\ t = _t ==> 
-      let pms = decrypt PCA.V.sk _pv _c in
-       (in_dom (_h, (pms, _t)) Find.m <=> res = Some pms) /\
-       (res <> None => res = Some pms) ] = 1%r.
+      let maybe = decrypt _pv PCA.V.sk _c in
+       res = 
+       if (in_dom ((_pv, _h), (proj maybe, _t)) Find.m) then maybe
+       else None ] = 1%r.
   proof.
-    progress; fun; sp.
+    fun; sp.
     while  
-     (let pms = decrypt PCA.V.sk pv c in
-      (forall x, mem x q => in_dom x Find.m) /\
-      (forall x, 
-       in_dom x Find.m => !mem x q => maybe_pms = None => 
-       x <> (h, (pms, t))) /\
-      (maybe_pms <> None => 
-       in_dom (h, (pms, t)) Find.m /\ 
-       maybe_pms = Some pms /\ h = h' /\  t = t'))
+     ((forall x, mem x q => in_dom x Find.m) /\
+      let maybe = decrypt pv PCA.V.sk c in
+        (maybe_pms <> None => 
+         maybe_pms = maybe /\ maybe <> None /\ 
+         in_dom ((pv, h), (proj maybe, t)) Find.m) /\
+        forall pv_ h_ pms_ t_, 
+          in_dom ((pv_, h_), (pms_, t_)) Find.m => 
+          !mem ((pv_, h_), (pms_, t_)) q => 
+          maybe_pms = None => 
+          ((pv_, h_), (maybe, t_)) <> ((pv, h), (Some pms_, t)))
      (card q).
-      intros z; sp; wp. 
+    intros z; sp; wp. 
       exists * pms, pv, c; elim *; intros pms pv c.
-      by call (check_spec pms pv c); skip; progress; smt. 
-    by wp; skip; progress; smt.
+      by call (check_spec pv pms c); skip; progress; smt.
+    wp; skip; intros &1; progress => //.
+      by smt.
+      by smt.
+      case (decrypt pv PCA.V.sk c = None){1} => ?.
+        by smt.
+        cut : (decrypt pv PCA.V.sk c = 
+               Some (proj (decrypt pv PCA.V.sk c))){1} by smt.
+        by smt.
   qed.
-  
-  local equiv RCCA2_Find_extract_guess : 
-    RCCA2.O1.extract ~ Find(O).O1.extract :
+
+  local equiv RCCA4_Find_extract_guess : 
+    RCCA4.O1.extract ~ Find(O).O1.extract :
     ={p, s} /\ ={V.keys, V.labels, V.guess, V.t, V.c} /\
     V.pk{1} = Find.pk{2} /\
     V.sk{1} = PCA.V.sk{2} /\ 
-    RCCA2.m{1} = Find.m{2} /\ 
-    RCCA2.d{1} = Find.d{2} /\
-    decrypt V.sk{1} (fst pp) V.c{1} = V.pms{1}
+    RCCA4.m{1} = Find.m{2} /\ 
+    RCCA4.d{1} = Find.d{2} /\
+    decrypt (fst pp) V.sk{1} V.c{1} = Some V.pms{1}
     ==>
     ={res} /\ ={V.keys, V.labels, V.guess, V.t, V.c} /\
     V.pk{1} = Find.pk{2} /\
     V.sk{1} = PCA.V.sk{2} /\ 
-    RCCA2.m{1} = Find.m{2} /\ 
-    RCCA2.d{1} = Find.d{2} /\
-    decrypt V.sk{1} (fst pp) V.c{1} = V.pms{1}. 
+    RCCA4.m{1} = Find.m{2} /\ 
+    RCCA4.d{1} = Find.d{2} /\
+    decrypt (fst pp) V.sk{1} V.c{1} = Some V.pms{1}. 
   proof.
     fun.
     sp; if => //.
@@ -1462,34 +2252,34 @@ section.
        (={pms, t, p, s, V.keys, V.labels, V.guess, V.t, V.c} /\
         V.pk{1} = Find.pk{2} /\
         V.sk{1} = PCA.V.sk{2} /\ 
-        RCCA2.m{1} = Find.m{2} /\ 
-        RCCA2.d{1} = Find.d{2} /\
-        decrypt V.sk{1} (fst pp) V.c{1} = V.pms{1} /\ 
-        ((in_dom t RCCA2.d /\ 
-          let (ms, pv, h, c) = proj RCCA2.d.[t] in 
-            p = h /\ decrypt V.sk pv c = pms){1} <=> 
-         (in_dom t Find.d /\ p = h /\ found){2})).
+        RCCA4.m{1} = Find.m{2} /\ 
+        RCCA4.d{1} = Find.d{2} /\
+        decrypt (fst pp) V.sk{1} V.c{1} = Some V.pms{1} /\ 
+        ((in_dom t RCCA4.d /\ 
+          let (ms, pv, h, c) = proj RCCA4.d.[t] in 
+            p = (pv, h) /\ decrypt pv V.sk c = Some pms){1} <=> 
+         (in_dom t Find.d /\ p = (pv, h) /\ found){2})).
         sp; exists * pms{2}, pv{2}, c{2}; elim *; intros pms pv c.
-        by call{2} (check_spec pms pv c); skip; progress; smt.
+        by call{2} (check_spec pv pms c); skip; progress; smt.
         by if => //; wp; try rnd; skip; progress.
       by wp.
   qed.
   
-  local equiv RCCA2_Find_dec_guess : 
-    RCCA2.O2.dec ~ Find(O).O2.dec :
+  local equiv RCCA4_Find_dec_guess : 
+    RCCA4.O2.dec ~ Find(O).O2.dec :
     ={p, t, c} /\ ={V.keys, V.labels, V.guess, V.t, V.c} /\
     V.pk{1} = Find.pk{2} /\
     V.sk{1} = PCA.V.sk{2} /\ 
-    RCCA2.m{1} = Find.m{2} /\ 
-    RCCA2.d{1} = Find.d{2} /\
-    decrypt V.sk{1} (fst pp) V.c{1} = V.pms{1} 
+    RCCA4.m{1} = Find.m{2} /\ 
+    RCCA4.d{1} = Find.d{2} /\
+    decrypt (fst pp) V.sk{1} V.c{1} = Some V.pms{1} 
     ==>
     ={res} /\ ={V.keys, V.labels, V.guess, V.t, V.c} /\
     V.pk{1} = Find.pk{2} /\
     V.sk{1} = PCA.V.sk{2} /\ 
-    RCCA2.m{1} = Find.m{2} /\ 
-    RCCA2.d{1} = Find.d{2} /\
-    decrypt V.sk{1} (fst pp) V.c{1} = V.pms{1}. 
+    RCCA4.m{1} = Find.m{2} /\ 
+    RCCA4.d{1} = Find.d{2} /\
+    decrypt (fst pp) V.sk{1} V.c{1} = Some V.pms{1}. 
   proof.
     fun.
     sp; if => //.
@@ -1499,36 +2289,38 @@ section.
       ={maybe_k, pv, h, p, t, c, V.labels, V.keys, V.guess, V.t, V.c} /\
       V.pk{1} = Find.pk{2} /\
       V.sk{1} = PCA.V.sk{2} /\
-      RCCA2.m{1} = Find.m{2} /\ 
-      RCCA2.d{1} = Find.d{2} /\
-      decrypt V.sk{1} (fst pp) V.c{1} = V.pms{1} /\
-      !(V.guess /\ same_key V.pk (fst pp) pv c /\ h = snd pp /\ t = V.t /\ V.c = c){1} /\
-      ((in_dom (h, (decrypt V.sk pv c, t)) RCCA2.m){1} <=> 
+      RCCA4.m{1} = Find.m{2} /\ 
+      RCCA4.d{1} = Find.d{2} /\
+      decrypt (fst pp) V.sk{1} V.c{1} = Some V.pms{1} /\
+      !(V.guess /\ (pv,h) = pp /\ t = V.t /\ V.c = c){1} /\
+      ((decrypt pv V.sk c <> None /\ 
+       in_dom ((pv, h), (proj (decrypt pv V.sk c), t)) RCCA4.m){1} <=> 
        maybe_pms{2} <> None) /\
       (maybe_pms <> None => 
-       maybe_pms = Some (decrypt PCA.V.sk pv c)){2}).
+       maybe_pms = Some (proj (decrypt pv PCA.V.sk c))){2}).
       sp; exists * pv{2}, c{2}, h{2}, t{2}; elim *; intros pv c h t.
-      by call{2} (find_spec pv c h t); skip; progress; smt.  
+      call{2} (find_spec pv c h t); skip; progress => //;
+        try rewrite some_proj; smt.
       if => //.
         by wp; skip; smt.
         by wp; rnd.
   qed.
 
-  local equiv RCCA2_Find_extract_choose : 
-    RCCA2.O1.extract ~ Find(O).O1.extract :
+  local equiv RCCA4_Find_extract_choose : 
+    RCCA4.O1.extract ~ Find(O).O1.extract :
     ={p, s} /\ ={V.keys, V.labels, V.guess, V.t} /\ !V.guess{1} /\
     V.pk{1} = Find.pk{2} /\
     V.sk{1} = PCA.V.sk{2} /\ 
-    RCCA2.m{1} = Find.m{2} /\ 
-    RCCA2.d{1} = Find.d{2} /\
-    decrypt V.sk{1} (fst pp) V.c{1} = V.pms{1}
+    RCCA4.m{1} = Find.m{2} /\ 
+    RCCA4.d{1} = Find.d{2} /\
+    decrypt (fst pp) V.sk{1} V.c{1} = Some V.pms{1}
     ==>
     ={res} /\ ={V.keys, V.labels, V.guess, V.t} /\ !V.guess{1} /\
     V.pk{1} = Find.pk{2} /\
     V.sk{1} = PCA.V.sk{2} /\ 
-    RCCA2.m{1} = Find.m{2} /\ 
-    RCCA2.d{1} = Find.d{2} /\
-    decrypt V.sk{1} (fst pp) V.c{1} = V.pms{1}. 
+    RCCA4.m{1} = Find.m{2} /\ 
+    RCCA4.d{1} = Find.d{2} /\
+    decrypt (fst pp) V.sk{1} V.c{1} = Some V.pms{1}. 
   proof.
     fun.
     sp; if => //.
@@ -1536,36 +2328,36 @@ section.
        (={pms, t, p, s, V.keys, V.labels, V.guess, V.t} /\ !V.guess{1} /\
         V.sk{1} = PCA.V.sk{2} /\ 
         V.pk{1} = Find.pk{2} /\
-        RCCA2.m{1} = Find.m{2} /\ 
-        RCCA2.d{1} = Find.d{2} /\
-        decrypt V.sk{1} (fst pp) V.c{1} = V.pms{1} /\ 
-        ((in_dom t RCCA2.d /\ 
-          let (ms, pv, h, c) = proj RCCA2.d.[t] in 
-            p = h /\ decrypt V.sk pv c = pms){1} <=> 
-         (in_dom t Find.d /\ p = h /\ found){2})).
+        RCCA4.m{1} = Find.m{2} /\ 
+        RCCA4.d{1} = Find.d{2} /\
+        decrypt (fst pp) V.sk{1} V.c{1} = Some V.pms{1} /\ 
+        ((in_dom t RCCA4.d /\ 
+          let (ms, pv, h, c) = proj RCCA4.d.[t] in 
+            p = (pv, h) /\ decrypt pv V.sk c = Some pms){1} <=> 
+         (in_dom t Find.d /\ p = (pv, h) /\ found){2})).
         sp; exists * pms{2}, pv{2}, c{2}; elim *; intros pms pv c.
-        by call{2} (check_spec pms pv c); skip; progress; smt.
+        by call{2} (check_spec pv pms c); skip; progress; smt.
         by if => //; wp; try rnd; skip; progress.
       by wp.
   qed.
 
-  local equiv RCCA2_Find_dec_choose : 
-    RCCA2.O2.dec ~ Find(O).O2.dec :
+  local equiv RCCA4_Find_dec_choose : 
+    RCCA4.O2.dec ~ Find(O).O2.dec :
     ={p, t, c} /\ ={V.keys, V.labels, V.guess, V.t} /\
     !V.guess{1} /\
     V.pk{1} = Find.pk{2} /\
     V.sk{1} = PCA.V.sk{2} /\ 
-    RCCA2.m{1} = Find.m{2} /\ 
-    RCCA2.d{1} = Find.d{2} /\
-    decrypt V.sk{1} (fst pp) V.c{1} = V.pms{1} 
+    RCCA4.m{1} = Find.m{2} /\ 
+    RCCA4.d{1} = Find.d{2} /\
+    decrypt (fst pp) V.sk{1} V.c{1} = Some V.pms{1} 
     ==>
     ={res} /\ ={V.keys, V.labels, V.guess, V.t} /\
     !V.guess{1} /\
     V.pk{1} = Find.pk{2} /\
     V.sk{1} = PCA.V.sk{2} /\ 
-    RCCA2.m{1} = Find.m{2} /\ 
-    RCCA2.d{1} = Find.d{2} /\
-    decrypt V.sk{1} (fst pp) V.c{1} = V.pms{1}. 
+    RCCA4.m{1} = Find.m{2} /\ 
+    RCCA4.d{1} = Find.d{2} /\
+    decrypt (fst pp) V.sk{1} V.c{1} = Some V.pms{1}. 
   proof.
     fun.
     sp; if => //.
@@ -1576,119 +2368,106 @@ section.
       !V.guess{1} /\
       V.pk{1} = Find.pk{2} /\
       V.sk{1} = PCA.V.sk{2} /\
-      RCCA2.m{1} = Find.m{2} /\ 
-      RCCA2.d{1} = Find.d{2} /\
-      decrypt V.sk{1} (fst pp) V.c{1} = V.pms{1} /\
-      !(V.guess /\ same_key V.pk (fst pp) pv c /\ h = snd pp /\ t = V.t /\ V.c = c){1} /\
-      ((in_dom (h, (decrypt V.sk pv c, t)) RCCA2.m){1} <=> 
+      RCCA4.m{1} = Find.m{2} /\ 
+      RCCA4.d{1} = Find.d{2} /\
+      decrypt (fst pp) V.sk{1} V.c{1} = Some V.pms{1} /\
+      !(V.guess /\ p = pp /\ t = V.t /\ V.c = c){1} /\
+      ((decrypt pv V.sk c <> None /\
+        in_dom ((pv, h), (proj (decrypt pv V.sk c), t)) RCCA4.m){1} <=> 
        maybe_pms{2} <> None) /\
       (maybe_pms <> None => 
-       maybe_pms = Some (decrypt PCA.V.sk pv c)){2}).
+       maybe_pms = Some (proj (decrypt pv PCA.V.sk c))){2}).
       sp; exists * pv{2}, c{2}, h{2}, t{2}; elim *; intros pv c h t.
-      by call{2} (find_spec pv c h t); skip; progress; smt.  
+      by call{2} (find_spec pv c h t); skip; progress; 
+        try rewrite some_proj; smt.  
       if => //.
         by wp; skip; smt.
         by wp; rnd.
   qed.
 
-  local equiv RCCA2_OW_PCA0 :
-    RCCA2.main ~ OW_PCA0.main :
-    true ==> (exists t, in_dom (snd pp, (V.pms, t)) RCCA2.m){1} => res{2}.
+  local equiv RCCA4_OW_PCA0 :
+    RCCA4.main ~ OW_PCA0.main :
+    true ==> (exists t, in_dom (pp, (V.pms, t)) RCCA4.m){1} => res{2}.
   proof.
-   fun.
-   inline OW_PCA0.B.choose OW_PCA0.B.guess.
-   swap{2} [4..8] -1; wp.
-   seq 6 8 :
-     (={V.keys, V.labels, V.guess, V.t} /\ !V.guess{1} /\
-      RCCA2.m{1} = Find.m{2} /\ RCCA2.d{1} = Find.d{2} /\
-      V.pk{1} = Find.pk{2} /\ V.sk{1} = PCA.V.sk{2} /\ 
-      pk0{2} = pk{2} /\ pk{2} = Find.pk{2} /\
-      V.pms{1} = k{2} /\ V.c{1} = c{2} /\ 
-      (decrypt V.sk (fst pp) V.c = V.pms){1}).
-   seq 5 6 : (={V.keys, V.labels, V.guess, V.t} /\ !V.guess{1} /\
-      RCCA2.m{1} = Find.m{2} /\ RCCA2.d{1} = Find.d{2} /\
-      V.sk{1} = PCA.V.sk{2} /\ pk0{2} = pk{2} /\ V.pk{1} = pk{2} /\
-      keypair(V.pk, V.sk){1}).
-   by inline V.init; wp; call keygen_spec_rel; call (_:true).
-   exists * V.sk{1}, V.pk{1}; elim *; intros sk pk.
-   call (enc_spec_rel sk pk (fst pp)); wp; skip; progress; smt.
-
-   seq 6 9 : (={V.keys, V.labels, V.guess, V.t, V.c} /\
-    V.pk{1} = Find.pk{2} /\ V.sk{1} = PCA.V.sk{2} /\ 
-    pk0{2} = pk{2} /\ pk{2} = Find.pk{2} /\
-    V.pms{1} = k{2} /\ V.c{2} = c0{2} /\ 
-    RCCA2.m{1} = Find.m{2} /\ 
-    RCCA2.d{1} = Find.d{2} /\
-    (decrypt V.sk (fst pp) V.c = V.pms){1}).
-   call (_: ={V.keys, V.labels, V.guess, V.t, V.c} /\
-    V.pk{1} = Find.pk{2} /\
-    V.sk{1} = PCA.V.sk{2} /\ 
-    RCCA2.m{1} = Find.m{2} /\ 
-    RCCA2.d{1} = Find.d{2} /\
-    (decrypt V.sk (fst pp) V.c = V.pms){1}).
-     by apply RCCA2_Find_dec_guess.
-     by apply RCCA2_Find_extract_guess.
-    wp; rnd; rnd; wp.
-   call (_: ={V.keys, V.labels, V.guess, V.t} /\ !V.guess{1} /\
-    V.pk{1} = Find.pk{2} /\
-    V.sk{1} = PCA.V.sk{2} /\ 
-    RCCA2.m{1} = Find.m{2} /\ 
-    RCCA2.d{1} = Find.d{2} /\
-    (decrypt V.sk (fst pp) V.c = V.pms){1}).
-     by apply RCCA2_Find_dec_choose.
-     by apply RCCA2_Find_extract_choose.
-   skip; progress.
-
+    fun.
+    inline OW_PCA0.B.choose OW_PCA0.B.guess.
+    swap{2} 7 -4; swap{2} [9..10] -5; swap{2} [7..8] -1; wp.
+    seq 6 8 :
+      (={V.keys, V.labels, V.guess, V.t} /\ !V.guess{1} /\
+       RCCA4.m{1} = Find.m{2} /\ RCCA4.d{1} = Find.d{2} /\
+       V.pk{1} = pk{2} /\ V.sk{1} = PCA.V.sk{2} /\ 
+       pk0{2} = pk{2} /\ pk{2} = Find.pk{2} /\
+       V.pms{1} = k{2} /\ V.c{1} = c{2} /\ 
+       (decrypt (fst pp) V.sk V.c = Some V.pms){1}).
+    seq 5 5 : (={V.keys, V.labels, V.guess, V.t} /\ !V.guess{1} /\
+       RCCA4.m{1} = Find.m{2} /\ RCCA4.d{1} = Find.d{2} /\
+       V.pk{1} = pk{2} /\ V.sk{1} = PCA.V.sk{2} /\ keypair(V.pk, V.sk){1}).
+    by inline V.init; wp; call keygen_spec_rel; call (_:true).
+    sp; exists * V.sk{1}, V.pk{1}; elim *; intros sk pk.
+    by call (enc_spec_rel sk pk (fst pp)); wp; skip; progress; smt.
+    seq 6 8 : (={V.keys, V.labels, V.guess, V.t, V.c} /\
+     V.pk{1} = Find.pk{2} /\ V.sk{1} = PCA.V.sk{2} /\ 
+     pk0{2} = pk{2} /\ pk{2} = Find.pk{2} /\
+     V.pms{1} = k{2} /\ V.c{2} = c0{2} /\ 
+     RCCA4.m{1} = Find.m{2} /\ 
+     RCCA4.d{1} = Find.d{2} /\
+     (decrypt (fst pp) V.sk V.c = Some V.pms){1}).
+    call (_: ={V.keys, V.labels, V.guess, V.t, V.c} /\
+     V.pk{1} = Find.pk{2} /\
+     V.sk{1} = PCA.V.sk{2} /\ 
+     RCCA4.m{1} = Find.m{2} /\ 
+     RCCA4.d{1} = Find.d{2} /\
+     (decrypt (fst pp) V.sk V.c = Some V.pms){1}).
+      by apply RCCA4_Find_dec_guess.
+      by apply RCCA4_Find_extract_guess.
+     wp; rnd; rnd; wp.
+    call (_: ={V.keys, V.labels, V.guess, V.t} /\ !V.guess{1} /\
+     V.pk{1} = Find.pk{2} /\
+     V.sk{1} = PCA.V.sk{2} /\ 
+     RCCA4.m{1} = Find.m{2} /\ 
+     RCCA4.d{1} = Find.d{2} /\
+     (decrypt (fst pp) V.sk V.c = Some V.pms){1}).
+      by apply RCCA4_Find_dec_choose.
+      by apply RCCA4_Find_extract_choose.
+    by wp.
     wp; exists * c0{2}; elim *; intros c.
     call{2} (find_any_spec (fst pp) c).
     by wp; skip; progress; smt.
   qed.
   
-  local lemma Pr_RCCA2_OW_PCA : forall &m,
-    Pr[RCCA2.main() @ &m : exists t, in_dom (snd pp, (V.pms, t)) RCCA2.m] <=
+  local lemma Pr_RCCA4_OW_PCA &m :
+    Pr[RCCA4.main() @ &m : exists t, in_dom (pp, (V.pms, t)) RCCA4.m] <=
     Pr[PCA.OW_PCA(PMS_KEM, B).main() @ &m : res].
   proof.
-    intros &m.
     apply (Trans _ Pr[OW_PCA0.main() @ &m : res]).
-    by equiv_deno RCCA2_OW_PCA0.
+    by equiv_deno RCCA4_OW_PCA0.
     by equiv_deno OW_PCA0_OW_PCA.
   qed.
-  
-  
-  (** RCCA2 -> NR *)
 
-  (* REMARK: the condition !mem t labels in the decryption oracle in
-   * the RCCA game could be dropped. A similar reduction to NR-PCA
-   * would work, but the map d would no longer be functional on t, and so
-   * the NR adversary would have to choose one decryption query for the
-   * challenge label at random, incurring a q_dec loss factor.
-   *)
+  (** RCCA4 -> NR *)
 
+  (* Adversary used in the reduction to NR_PCA *)
   local module C(PCO:PCA.Oracle) = {
     module F = Find(PCO)
     module A = A(Find(PCO).O1, Find(PCO).O2)
       
-    fun choose(pk:pkey) : version = {
-      var t : label;
-      V.init();
-      Find.m = Core.empty;
-      Find.d = Core.empty;
-      Find.pk = pk;
-      V.t = A.choose(pk);
-      return (fst pp);
-    }
+    fun choose(pk:pkey) : unit = { Find.pk = pk; }
   
-    fun guess(c:ciphertext) : version * ciphertext = {
+    fun guess(c:ciphertext) : ciphertext = {
       var pms : pms;
       var k0, k1 : ms;
       var b' : bool;
+      V.init();
       V.c = c;
+      Find.m = Core.empty;
+      Find.d = Core.empty;
+      V.t = A.choose(Find.pk);
       k0 = $key;
       k1 = $key;
       V.keys = add k0 (add k1 V.keys);
       V.guess = true;
       b' = A.guess(c, k0);
-      return let (k, pv, h, c) = proj Find.d.[V.t] in (pv, c);
+      return let (k, pv, h, c) = proj Find.d.[V.t] in c;
     }
   }.
 
@@ -1697,16 +2476,17 @@ section.
     
     fun main() : bool = {
       var pk : pkey;
-      var t, t' : version;
-      var k, k' : pms;
+      var p : version;
+      var k : pms;
+      var maybe_k : pms option;
       var c, c' : ciphertext;
       PMS_KEM.init();
       (pk, PCA.V.sk) = PMS_KEM.keygen();
-      (k, c) = PMS_KEM.enc((), pk, fst pp);
-      t = C.choose(pk);
-      (t', c') = C.guess(c);
-      k' = PMS_KEM.dec((), PCA.V.sk, t', c');
-      return (c <> c' /\ k' = k);
+      (k, c) = PMS_KEM.enc(fst pp, pk, ());
+      C.choose(pk);
+      c' = C.guess(c);
+      maybe_k = PMS_KEM.dec(fst pp, PCA.V.sk, (), c');
+      return (c <> c' /\ maybe_k = Some k);
     }
   }.
 
@@ -1717,121 +2497,117 @@ section.
     swap{1} 3 1.
     inline PCA.NR_PCA(PMS_KEM, C).A.guess NR_PCA0.C.guess.
     call (_: ={glob Find, glob PCA.V}); wp.
-    call (_: ={glob Find, glob PCA.V}).
-      fun.
-      eqobs_in true (={glob PCA.V}) : (={maybe_k, glob Find, glob PCA.V}).
-      apply OW_PCA0_OW_PCA_check.
-      fun.
-      eqobs_in (={glob PCA.V}) true : (={k, glob Find, glob PCA.V}).
-      apply OW_PCA0_OW_PCA_check.
-    seq 3 3 : 
-     (={pk, glob PCA.V, glob A, glob Find, t} /\ 
-      t{1} = fst pp /\ keypair(pk, PCA.V.sk){2}).
+    eqobs_in true (={glob PCA.V}) : (={k,c,glob Find,glob PCA.V}).
+    by apply OW_PCA0_OW_PCA_check.
+    progress.
+      by cut X : forall x, tt = x by smt; apply X.
+      by apply stateless_pms_kem.
+    seq 3 3 : (={pk,Find.pk,glob PCA.V} /\ 
+      keypair(pk, PCA.V.sk){2} /\ pk{1} = Find.pk{1}).
     inline PCA.NR_PCA(PMS_KEM, C).A.choose NR_PCA0.C.choose; wp.
-    call (_: ={glob PCA.V, glob Find}) => //.
-      fun.
-      eqobs_in true (={glob PCA.V}) : (={maybe_k, glob Find, glob PCA.V}).
-      apply OW_PCA0_OW_PCA_check.
-      fun.
-      eqobs_in (={glob PCA.V}) true : (={k, glob Find, glob PCA.V}).
-      apply OW_PCA0_OW_PCA_check.
-    by inline V.init; wp; call keygen_spec_rel; call (_:true).
-    wp; rnd; rnd; wp.
-    exists * PCA.V.sk{1}, pk{1}, t{1}; elim *; intros sk pk t.
-    by call (enc_spec_rel sk pk t); skip; progress; smt.
+    call keygen_spec_rel; call (_:true).
+    skip; progress.
+    exists * PCA.V.sk{1}, pk{1}; elim *; intros sk pk.
+    call (enc_spec_rel sk pk (fst pp)); skip; progress.
+    cut X : forall x, tt = x by smt; apply X.
   qed.
   
-  local equiv RCCA2_NR :
-    RCCA2.main ~ NR_PCA0.main :
+  local equiv RCCA4_NR_PCA0 :
+    RCCA4.main ~ NR_PCA0.main :
     true ==> 
-    (let (k, pv, h, c) = proj RCCA2.d.[V.t] in
-       c <> V.c /\ decrypt V.sk pv c = V.pms){1} => res{2}.
+    (let (k, pv, h, c) = proj RCCA4.d.[V.t] in
+       pv = fst pp /\ h = snd pp /\ 
+       c <> V.c /\ decrypt pv V.sk c = Some V.pms){1} => res{2}.
   proof.
-   fun.
-   inline NR_PCA0.C.choose NR_PCA0.C.guess.
-   swap{2} [4..8] -1; wp.
-   seq 6 8 :
-     (={V.keys, V.labels, V.guess, V.t} /\ !V.guess{1} /\
-      RCCA2.m{1} = Find.m{2} /\ RCCA2.d{1} = Find.d{2} /\
-      V.sk{1} = PCA.V.sk{2} /\ 
-      V.pk{1} = pk{2} /\ pk0{2} = pk{2} /\ pk{2} = Find.pk{2} /\
-      V.pms{1} = k{2} /\ V.c{1} = c{2} /\ 
-      (decrypt V.sk (fst pp) V.c = V.pms){1}).
-   seq 5 7 : (={V.keys, V.labels, V.guess, V.t} /\ !V.guess{1} /\
-      RCCA2.m{1} = Find.m{2} /\ RCCA2.d{1} = Find.d{2} /\
-      V.sk{1} = PCA.V.sk{2} /\ 
-      V.pk{1} = pk{2} /\ pk0{2} = pk{2} /\ pk{2} = Find.pk{2} /\
-      keypair(V.pk, V.sk){1}).
-   by inline V.init; wp; call keygen_spec_rel; call (_:true).
-   exists * V.sk{1}, V.pk{1}; elim *; intros sk pk.
-   call (enc_spec_rel sk pk (fst pp)); wp; skip; progress; smt.
+    fun.
+    inline NR_PCA0.C.choose NR_PCA0.C.guess.
+    swap{2} 7 -4; swap{2} [9..10] -5; swap{2} [7..8] -1; wp.
+    seq 6 8 :
+      (={V.keys, V.labels, V.guess, V.t} /\ !V.guess{1} /\
+       RCCA4.m{1} = Find.m{2} /\ RCCA4.d{1} = Find.d{2} /\
+       V.pk{1} = pk{2} /\ V.sk{1} = PCA.V.sk{2} /\ 
+       pk0{2} = pk{2} /\ pk{2} = Find.pk{2} /\
+       V.pms{1} = k{2} /\ V.c{1} = c{2} /\ 
+       (decrypt (fst pp) V.sk V.c = Some V.pms){1}).
+     seq 5 5 : (={V.keys, V.labels, V.guess, V.t} /\ !V.guess{1} /\
+       RCCA4.m{1} = Find.m{2} /\ RCCA4.d{1} = Find.d{2} /\
+       V.pk{1} = pk{2} /\ V.sk{1} = PCA.V.sk{2} /\ keypair(V.pk, V.sk){1}).
+     by inline V.init; wp; call keygen_spec_rel; call (_:true).
+     sp; exists * V.sk{1}, V.pk{1}; elim *; intros sk pk.
+     by call (enc_spec_rel sk pk (fst pp)); wp; skip; progress; smt.
+    seq 6 8 : (={V.keys, V.labels, V.guess, V.t, V.c} /\
+     V.pk{1} = Find.pk{2} /\
+     V.sk{1} = PCA.V.sk{2} /\ V.c{2} = c0{2} /\ c{2} = c0{2} /\ pk0{2} = pk{2} /\
+     V.pms{1} = k{2} /\ 
+     RCCA4.m{1} = Find.m{2} /\ 
+     RCCA4.d{1} = Find.d{2} /\
+     (decrypt (fst pp) V.sk V.c = Some V.pms){1}).
+    call (_: ={V.keys, V.labels, V.guess, V.t, V.c} /\
+     V.pk{1} = Find.pk{2} /\
+     V.sk{1} = PCA.V.sk{2} /\ 
+     RCCA4.m{1} = Find.m{2} /\ 
+     RCCA4.d{1} = Find.d{2} /\
+     (decrypt (fst pp) V.sk V.c = Some V.pms){1}).
+      by apply RCCA4_Find_dec_guess.
+      by apply RCCA4_Find_extract_guess.
+     wp; rnd; rnd; wp.
+    call (_: ={V.keys, V.labels, V.guess, V.t} /\ !V.guess{1} /\
+     V.pk{1} = Find.pk{2} /\
+     V.sk{1} = PCA.V.sk{2} /\ 
+     RCCA4.m{1} = Find.m{2} /\ 
+     RCCA4.d{1} = Find.d{2} /\
+     (decrypt (fst pp) V.sk V.c = Some V.pms){1}).
+      by apply RCCA4_Find_dec_choose.
+      by apply RCCA4_Find_extract_choose.
+    by wp.
 
-   seq 6 9 : (={V.keys, V.labels, V.guess, V.t, V.c} /\
-    V.pk{1} = Find.pk{2} /\
-    V.sk{1} = PCA.V.sk{2} /\ V.c{2} = c0{2} /\ c{2} = c0{2} /\ pk0{2} = pk{2} /\
-    V.pms{1} = k{2} /\ 
-    RCCA2.m{1} = Find.m{2} /\ 
-    RCCA2.d{1} = Find.d{2} /\
-    (decrypt V.sk (fst pp) V.c = V.pms){1}).
-   call (_: ={V.keys, V.labels, V.guess, V.t, V.c} /\
-    V.pk{1} = Find.pk{2} /\
-    V.sk{1} = PCA.V.sk{2} /\ 
-    RCCA2.m{1} = Find.m{2} /\ 
-    RCCA2.d{1} = Find.d{2} /\
-    (decrypt V.sk (fst pp) V.c = V.pms){1}).
-     by apply RCCA2_Find_dec_guess.
-     by apply RCCA2_Find_extract_guess.
-    wp; rnd; rnd; wp.
-   call (_: ={V.keys, V.labels, V.guess, V.t} /\ !V.guess{1} /\
-    V.pk{1} = Find.pk{2} /\
-    V.sk{1} = PCA.V.sk{2} /\ 
-    RCCA2.m{1} = Find.m{2} /\ 
-    RCCA2.d{1} = Find.d{2} /\
-    (decrypt V.sk (fst pp) V.c = V.pms){1}).
-     by apply RCCA2_Find_dec_choose.
-     by apply RCCA2_Find_extract_choose.
-   skip; progress.
-
-    sp; wp; exists * PCA.V.sk{2}, t'{2}, c'{2}; elim *; intros sk pv c.
-    call{2} (dec_spec sk pv c).
-    by skip; progress; smt.
+    sp; wp; exists * PCA.V.sk{2}, c'{2}; elim *; intros sk c.
+    call{2} (dec_spec sk (fst pp) c).
+    by skip; smt.
   qed.
   
-  local lemma Pr_RCCA2_NR_PCA : forall &m,
-    Pr[RCCA2.main() @ &m : let (k, pv, h, c) = proj RCCA2.d.[V.t] in
-       c <> V.c /\ decrypt V.sk pv c = V.pms] <=
+  local lemma Pr_RCCA4_NR_PCA &m :
+    Pr[RCCA4.main() @ &m : let (k, pv, h, c) = proj RCCA4.d.[V.t] in
+       pv = fst pp /\ h = snd pp /\ c <> V.c /\ decrypt pv V.sk c = Some V.pms] <=
     Pr[PCA.NR_PCA(PMS_KEM, C).main() @ &m : res].
   proof.
-    intros &m.
     apply (Trans _ Pr[NR_PCA0.main() @ &m : res]).
-    by equiv_deno RCCA2_NR.
+    by equiv_deno RCCA4_NR_PCA0.
     by equiv_deno NR_PCA0_NR_PCA.
   qed.
-  
+
   (** Conclusion **)
-  lemma Conclusion : forall &m,
-    exists (B <: PCA.OW_Adversary {PCA.V}) 
-           (C <: PCA.NR_Adversary {PCA.V}),
-     Pr[RCCA(KEM(RO_KEF, PMS_KEM), A(RO_KEF)).main() @ &m : res] - 1%r / 2%r <=
-     Pr[PCA.OW_PCA(PMS_KEM, B).main() @ &m : res] +
-     Pr[PCA.NR_PCA(PMS_KEM, C).main() @ &m : res].
+  module RCCA = Outer_KEM.RCCA.RCCA.
+
+  lemma Conclusion &m :
+    exists (B <: PCA.OW_Adversary {PCA.V}) (C <: PCA.NR_Adversary {PCA.V}),
+      Pr[RCCA(KEM(RO_KEF, PMS_KEM), A(RO_KEF)).main() @ &m : res] - 1%r / 2%r <=
+      qKEF%r / (card (toFSet univ<:pms>))%r +
+      Pr[PCA.OW_PCA(PMS_KEM, B).main() @ &m : res] +
+      Pr[PCA.NR_PCA(PMS_KEM, C).main() @ &m : res].
   proof.
-    intros &m; exists B, C.
-    cut X : forall (x y z), 0%r <= z => x <= y + z => x - y <= z by smt.
-    apply X; first by smt.
-    apply (Trans _ (1%r / 2%r + Pr[RCCA1.main() @ &m : RCCA1.abort]));
-    first by apply (Pr_RCCA_RCCA1 &m).
+    exists B, C.
+    cut X : forall (x y z:real), x <= y + z => x - y <= z by smt.
+    apply X.
+    apply (Trans _ (1%r / 2%r + 
+      (Pr[RCCA2.main() @ &m : exists pv h t, in_dom ((pv, h), (proj RCCA2.fake.[(pv, t)], t)) RCCA2.m] +
+      Pr[RCCA3.main() @ &m : RCCA3.abort]))).
+    cut W := Pr_RCCA_RCCA3 &m; smt.
     apply addleM => //.
+    cut -> : forall (x y z:real), x + y + z = x + (y + z) by smt.
+    apply addleM => //.
+    apply (Pr_RCCA2 &m).
     apply (Trans _
-      (Pr[RCCA2.main() @ &m : exists t, in_dom (snd pp, (V.pms, t)) RCCA2.m] +  
-       Pr[RCCA2.main() @ &m : let (k, pv, h, c) = proj RCCA2.d.[V.t] in
-          c <> V.c /\ decrypt V.sk pv c = V.pms])).
-    by apply (Pr_RCCA1_RCCA2 &m).
+      (Pr[RCCA4.main() @ &m : exists t, in_dom (pp, (V.pms, t)) RCCA4.m] +  
+       Pr[RCCA4.main() @ &m : let (k, pv, h, c) = proj RCCA4.d.[V.t] in
+          pv = fst pp /\ h = snd pp /\ c <> V.c /\ decrypt pv V.sk c = Some V.pms])).
+    by apply (Pr_RCCA3_RCCA4 &m).
     apply addleM.
-      by apply (Pr_RCCA2_OW_PCA &m).
-      by apply (Pr_RCCA2_NR_PCA &m).
+      by apply (Pr_RCCA4_OW_PCA &m).
+      by apply (Pr_RCCA4_NR_PCA &m).
   qed.
 
 end section.
 
 print axiom Conclusion.
+print module type Adversary.
